Simplification of some proofs

theories/BI.v
@@ -8,6 +8,7 @@ Require Import brede_herbelin.
 Set Implicit Arguments.
 Unset Strict Implicit.
 Unset Printing Implicit Defensive.
+Require Import Lia.
 
 Set Bullet Behavior "Strict Subproofs".
 Set Default Goal Selector "!".
@@ -266,11 +267,12 @@ Proof.
 Qed.
 
 End ContinuousInduction.
+
+
 Section BarInduction.
 
-
   (*The aim of this Section is to prove that Sequential continuity + Bar Induction
-   implies Dialogue continuity.*)
+   implies Dialogue continuity for I = nat.*)
 Variable BI : forall A T, @BI_ind A T.
 Variable O A : Type.
 Notation I := nat.
@@ -485,16 +487,45 @@ Qed.
 
 End BarInduction.
 
-Section GeneralisedBarInduction.
 
+Section GeneralisedBarInduction.
+(*We generalize the previous result and aim to prove that 
+  Sequential continuity + Generalized Bar Induction 
+   implies Dialogue continuity for any type I with decidable equality.*)
 Variable I : eqType.
 Variables O A : Type.
 Implicit Type (F : (I -> O) -> A).
-Print GBI.
 Variable HGBI : forall T, @GBI I O T.
+
+(*We start with two small lemmas about Add that will be useful later on.*)
+
+Lemma Add_rcons {X : Type} (a : X) (l : seq X): List.Add a l (rcons l a).
+Proof.
+  induction l ; cbn.
+  - now econstructor.
+  - now econstructor.
+Qed.
+
+Lemma Add_cat {X : Type} (a : X) (u v w : seq X) :
+  List.Add a u v ->
+  List.Add a (u ++ w) (v ++ w).
+Proof.
+  induction 1 ; intros.
+  - rewrite - cat1s - catA cat1s.
+    now econstructor.
+  - rewrite - cat1s - (cat1s x l') - catA - catA cat1s cat1s.
+    now econstructor.
+Qed.
+
+(*We define is_fun_list, a predicate on lists u : seq (I * O)
+ describing the fact that u is a finite approximation of some
+ function f : I -> O.*)
 
 Definition is_fun_list (u : seq (I * O)) :=
   forall i j j', List.In (i, j) u -> List.In (i, j') u -> j = j'.
+
+(*Without much surprise, [seq (i, f i) | i <- u] for some list u : seq I
+ is a finite approximation of some function.*)
 
 Lemma is_fun_map (u : seq I) (f : I -> O) :
   is_fun_list [seq (i, f i) | i <- u].
@@ -507,6 +538,8 @@ Proof.
   apply aux in Hj, Hj' ; now subst.
 Qed.
 
+
+(*is_fun_list is downwards closed.*)
 Lemma is_fun_list_incl (u v : seq (I * O)) :
   is_fun_list v ->
   List.incl u v ->
@@ -516,6 +549,7 @@ Proof.
   apply Hincl in Hin, Hin' ; eapply Hfun ; eassumption.
 Qed.
 
+(*We can concatenate two finite approximations if their domains are disjoint.*)
 Lemma is_fun_cat_notin_dom (u v : seq (I * O))
   (Hu : is_fun_list u)
   (Hv : is_fun_list v)
@@ -547,7 +581,8 @@ Proof.
   now apply (in_map fst) in H ; cbn in H.
 Qed.
   
-  
+(*Some lemmas about adding elements at the beginning or the end 
+ of some finite approximation u.*)  
 Lemma is_fun_cons_notin_dom (u : seq (I * O)) (i : I) (o : O)
   (Hu : is_fun_list u)
   (H : ~ (List.In i (map fst u))) :
@@ -578,105 +613,15 @@ Proof.
   cbn ; intros [Heq | Hfalse] ; [ now apply Hnoteq | assumption].
 Qed.  
     
-
-
-Lemma NoDup_rcons {X : Type} (x : X) (l : seq X) :
-  List.NoDup l -> ~ List.In x l -> List.NoDup (rcons l x).
-Proof.
-  induction 1 as [| a l Hnotina k IHk ]; intros Hnotinx.
-  { apply List.NoDup_cons ; [assumption | now econstructor]. }
-  rewrite rcons_cons.
-  econstructor 2.
-  2:{ apply IHk ; intros Hin.
-      apply Hnotinx.
-      now cbn ; right.
-  }
-  rewrite <- cats1 ; intros Hin.
-  apply List.in_app_or in Hin ; destruct Hin as [Hinl | Hinx] ; [now apply Hnotina |].
-  cbn in Hinx ; destruct Hinx as [Heqxq | HFalse] ; [ subst | assumption].
-  apply Hnotinx ; now left.
-Qed.  
-
-Inductive indbarred_fun_list (T : seq (I * O) -> Prop) : seq (I * O) -> Prop :=
-| ieta_fun_list : forall u' u : seq (I * O),
-    T u -> List.incl u u' -> is_fun_list u' -> indbarred_fun_list T u'
-| ibeta_NoDup : forall (a : I) (v : seq (I * O)),
-    ~ List.In a [seq i.1 | i <- v] ->
-    (forall b : O, indbarred_fun_list T (v ++ [:: (a, b)])) ->
-    indbarred_fun_list T v.
-
-
-
-Lemma indbarred_indbarred_fun_list (T : seq (I * O) -> Prop) :
-  indbarred T nil ->
-  indbarred_fun_list T nil.
-Proof.
-  have aux: is_fun_list (@nil (I * O)).
-  { intros q r r' Hin ; now inversion Hin. }
-  revert aux ; generalize (@nil (I * O)) ; intros l Hfun Hyp ; revert Hfun.
-  induction Hyp as [u v Hv Hincl | i v Hnotin k IHk ] ; intros.
-  { econstructor ; eassumption. }
-  econstructor 2 ; [ now apply Hnotin |].
-  intros o ; apply IHk.
-  rewrite cats1 ; apply is_fun_rcons_notin_dom ; assumption.
-Qed.
-
-
-(*Inductive indbarred_NoDup (T : seq (I * O) -> Prop) : seq (I * O) -> Prop :=
-| ieta_NoDup : forall u' u : seq (I * O),
-    T u -> List.incl u u' -> List.NoDup (map fst u') -> indbarred_NoDup T u'
-| ibeta_NoDup : forall (a : I) (v : seq (I * O)),
-    ~ List.In a [seq i.1 | i <- v] ->
-    (forall b : O, indbarred_NoDup T (v ++ [:: (a, b)])) -> indbarred_NoDup T v.
-
-
-
-Lemma indbarred_indbarred_NoDup (T : seq (I * O) -> Prop) :
-  indbarred T nil ->
-  indbarred_NoDup T nil.
-Proof.
-  have aux: List.NoDup (map fst (@nil (I * O))) by (apply List.NoDup_nil).
-  revert aux ; generalize (@nil (I * O)) ; intros l HNoDup Hyp ; revert HNoDup.
-  induction Hyp as [u v Hv Hincl | i v Hnotin k IHk ] ; intros.
-  { econstructor ; eassumption. }
-  econstructor 2 ; [ now apply Hnotin |].
-  intros o ; apply IHk.
-  rewrite cats1.
-  rewrite map_rcons ; apply NoDup_rcons ; cbn ; assumption.
-Qed.
-  
-Lemma indbarred_NoDup_indbarred (T : seq (I * O) -> Prop) :
-  indbarred_NoDup T nil ->
-  indbarred T nil.
-Proof.
-  generalize (@nil (I * O)) ; intros l ; induction 1.
-  { now econstructor ; eassumption. }
-  econstructor 2 ; eassumption.
-Qed.
-*)
-
-
+(*Since we have finite approximations of functions,
+ we can consider them as partial functions, through eval_list.*)
 Fixpoint eval_list (u : seq (I * O)) (i : I) : option O :=
   match u with
   | nil => None
   | (i', o') :: v => if i == i' then Some o' else eval_list v i
   end.
 
-Fixpoint eval_ext_tree_aux_finapp
-  (tau : @ext_tree I O A) (u: seq (I * O)) (n : nat) (l : seq O)
-  {struct n} : result :=
-  match n with
-  | 0 => tau l
-  | k.+1 =>
-      match tau l with
-      | ask q => match eval_list u q with
-                 | None => ask q
-                 | Some o => eval_ext_tree_aux_finapp tau u k (rcons l o)
-                 end
-      | output _ => tau l
-      end
-  end.
-
+(*Some lemmas about eval_list.*)
 Lemma eval_list_In u i o :
   eval_list u i = Some o ->
   List.In (i, o) u.
@@ -770,7 +715,6 @@ Proof.
     intros Heq ; now eapply IHu ; eauto.
 Qed.
 
-    
 Lemma eval_list_monotone (u v : seq (I * O)) (i : I) (o : O) :
   is_fun_list v ->
   List.incl u v ->
@@ -792,7 +736,65 @@ Proof.
   remember (eval_list u i) as aux ; destruct aux as [o | ] ; [ | reflexivity].
   erewrite (eval_list_monotone Hfun Hincl) in Heq ; [eassumption | eauto].
 Qed.
-  
+
+Lemma eval_list_map_In (alpha : I -> O) :
+  forall u i o, eval_list [seq (i, alpha i) | i <- u] i = Some o -> o = alpha i.
+Proof.
+  intros u i o H.
+  revert H ; induction u ; cbn ; intros ; [now inversion H | ].
+  destruct (@eqP I i a) ; subst ; [now inversion H | ].
+  now apply IHu.
+Qed.
+
+(*We now define evalueation of an extensional tree
+ using a finite approximation u : seq (I * O). *)
+
+Fixpoint eval_ext_tree_aux_finapp
+  (tau : @ext_tree I O A) (u: seq (I * O)) (n : nat) (l : seq O)
+  {struct n} : result :=
+  match n with
+  | 0 => tau l
+  | k.+1 =>
+      match tau l with
+      | ask q => match eval_list u q with
+                 | None => ask q
+                 | Some o => eval_ext_tree_aux_finapp tau u k (rcons l o)
+                 end
+      | output _ => tau l
+      end
+  end.
+
+(*If we first evaluate an extensional tree tau with a function f : I -> O and
+  reach an output, then we can evaluate tau with a finite approximation
+  built from the trace of the previous evaluation.
+ This will be useful to go from eval_ext_tree_aux to eval_ext_tree_aux_finapp
+ in the final theorem.*)
+
+Lemma eval_ext_tree_finapp_trace (tau : ext_tree) f n a l :
+  eval_ext_tree_aux tau f n l = output a ->
+  eval_ext_tree_aux_finapp tau [seq (i, f i) | i <- eval_ext_tree_trace_aux tau f n l] n l =
+    output a.
+Proof.
+  assert (aux := @is_fun_map (eval_ext_tree_trace_aux tau f n l) f) ; revert aux.
+  change (eval_ext_tree_trace_aux tau f n l) with (nil ++ (eval_ext_tree_trace_aux tau f n l)) at 1 2.
+  generalize (@nil I) as u ; revert l.
+  induction n as [ | n IHn] ; cbn in * ; intros l u aux Heq.
+  { destruct u ; cbn ; [assumption | now rewrite Heq ]. }
+  remember (tau l) as r ; destruct r ; cbn in *.
+  2: assumption.
+  erewrite <- cat_rcons ; erewrite <- cat_rcons in aux.
+  suff: eval_list [seq (i, f i) |
+                    i <- rcons u s ++ eval_ext_tree_trace_aux tau f n (rcons l (f s))] s =
+          Some (f s).
+  { intros Hyp ; rewrite Hyp.
+    specialize (IHn (rcons l (f s)) (rcons u s)) ; erewrite IHn ; eauto.
+  }
+  apply In_eval_list ; [assumption | eapply (in_map (fun i => (i, f i)))].
+  now rewrite - cats1 - catA cat1s ; eapply List.in_elt.
+Qed.  
+
+(*We now prove some technical lemmas proving that 
+ eval_ext_tree_aux_finapp is monotone in different ways.*)
 Lemma eval_ext_tree_aux_finapp_monotone_output_list
   (tau : @ext_tree I O A) (u v: seq (I * O)) (n : nat) (l : seq O) (a : A) :
   is_fun_list v ->
@@ -841,6 +843,21 @@ Proof.
 Qed.
 
 
+Lemma eval_ext_tree_aux_finapp_monotone_ask_fuel
+  (tau : @ext_tree I O A) (u : seq (I * O)) (n m : nat) (l : seq O) (q : I) :
+  is_fun_list u ->
+  eval_list u q = None ->
+  eval_ext_tree_aux_finapp tau u n l = ask q ->
+  eval_ext_tree_aux_finapp tau u (n + m) l = ask q.
+Proof.
+  revert u n l q.
+  induction n as [| k IHk] ; intros * Hfun Hnotin Heq ; cbn in *.
+  - destruct m ; cbn ; [ assumption | now rewrite Heq Hnotin ].
+  - destruct (tau l) ; cbn in * ; [ | now inversion Heq ].
+    destruct (eval_list u s) ; cbn in * ; [ | assumption].
+    now apply IHk.
+Qed.
+
 Lemma eval_ext_tree_aux_finapp_monotone_ask_list_nomorefuel
   (tau : @ext_tree I O A) (u v: seq (I * O)) (n : nat) (l : seq O) (q : I) (a : O) :
   is_fun_list v ->
@@ -859,208 +876,249 @@ Proof.
     rewrite Hnotin in Heqev ; now inversion Heqev.
 Qed.
 
-Lemma eval_ext_tree_aux_finapp_monotone_ask_fuel
-  (tau : @ext_tree I O A) (u : seq (I * O)) (n m : nat) (l : seq O) (q : I) :
-  is_fun_list u ->
-  eval_list u q = None ->
-  eval_ext_tree_aux_finapp tau u n l = ask q ->
-  eval_ext_tree_aux_finapp tau u (n + m) l = ask q.
-Proof.
-  revert u n l q.
-  induction n as [| k IHk] ; intros * Hfun Hnotin Heq ; cbn in *.
-  - destruct m ; cbn ; [ assumption | now rewrite Heq Hnotin ].
-  - destruct (tau l) ; cbn in * ; [ | now inversion Heq ].
-    destruct (eval_list u s) ; cbn in * ; [ | assumption].
-    now apply IHk.
-Qed.
+(*This lemma, a bit ad-hoc, proves that if the evaluation of some
+ extensional tree tau using an approximation u is blocked because 
+ of lack of fuel, although, the answer to the question is in u,
+ then raising the fuel will lead to the same computation step,
+ for any approximation v extending u.
+ *)
 
-Lemma eval_ext_tree_aux_finapp_one_step_fuel tau u v w l n q a :
+Lemma eval_ext_tree_aux_finapp_one_step_fuel tau u v l n q a :
   is_fun_list v ->
-  is_fun_list w ->
   List.incl u v ->
-  List.incl u w ->
   eval_list u q = Some a ->
   eval_ext_tree_aux_finapp tau u n l = ask q ->
-  eval_ext_tree_aux_finapp tau v n.+1 l = eval_ext_tree_aux_finapp tau w n.+1 l.
+  eval_ext_tree_aux_finapp tau u n.+1 l = eval_ext_tree_aux_finapp tau v n.+1 l.
 Proof.
-  revert u v w l q.
-  induction n as [ | n IHn] ; intros * Hfunv Hfunw Hinclv Hinclw Heval Hasku.
+  revert u v l q.
+  induction n as [ | n IHn] ; intros * Hfunv Hinclv Heval Hasku.
   - cbn in *.
-    rewrite Hasku.
-    now do 2 (erewrite eval_list_monotone ; eauto).
+    rewrite Hasku Heval.
+    now erewrite eval_list_monotone ; eauto.
   - cbn in *.
-    remember (tau l) as aux ; destruct aux as [i | r] ; subst ; [ | now inversion Hasku].
+    remember (tau l) as aux ; destruct aux as [i | r] ; subst ;
+      [ | now inversion Hasku].
     remember (eval_list u i) as aux2 ; destruct aux2 as [ o | ].
     2:{ inversion Hasku ; subst.
         rewrite Heval in Heqaux2 ; now inversion Heqaux2.
     }
-    now do 2 (erewrite eval_list_monotone ; eauto).
+    now erewrite eval_list_monotone ; eauto.
 Qed.
 
-Print indbarred_fun_list.
 
-Inductive indbarred_ext_tree (T : seq (I * O) -> Prop) (tau : ext_tree) :
-  seq (I * O) -> Prop :=
-|  ieta_ext_tree : forall (u' u : seq (I * O)) (r : A),
-    T u ->
-    List.incl u u' ->
-    is_fun_list u' ->
-    eval_ext_tree_aux_finapp tau u (size u) nil = output r ->
-    eval_ext_tree_aux_finapp tau u' (size u') nil = output r ->
-    indbarred_ext_tree T tau u'
-| isucc_ext_tree : forall (u : seq (I * O)) (q : I) (a : O),
-    is_fun_list u ->
-    eval_ext_tree_aux_finapp tau u (size u) nil = ask q ->
-    eval_list u q = Some a ->
-    indbarred_ext_tree T tau (u ++[:: (q, a)]) ->
-    indbarred_ext_tree T tau u
-| ibeta_ext_tree : forall (u : seq (I * O)) (q : I),
-    is_fun_list u ->
-    eval_ext_tree_aux_finapp tau u (size u) nil = ask q ->
-    eval_list u q = None ->
-    (forall o : O, indbarred_ext_tree T tau (u ++ [:: (q, o)])) ->
-    indbarred_ext_tree T tau u.
-
-
-Print Acc.
-
-Inductive goodRel (tau : ext_tree) : seq (I * O) -> seq (I *O) -> Prop :=
-| goodRel_in_dom u i i' o : is_fun_list u ->
-                          eval_ext_tree_aux_finapp tau u (size u) nil = ask i ->
-                          eval_list u i' = None ->
-                          goodRel tau (u ++ [:: (i', o)]) u
-| goodRel_notin_dom u i i' o : is_fun_list u ->
-                             eval_ext_tree_aux_finapp tau u (size u) nil = ask i ->
-                             eval_list u i' = Some o ->
-                             goodRel tau (u ++ [:: (i', o)]) u.
-
-Lemma hope (tau : ext_tree) (l : seq (I * O)) :
-  indbarred_fun_list
-    (fun u => exists n a, eval_ext_tree_aux_finapp tau u n nil = output a) l ->
-  Acc (goodRel tau) l.
+(*Let us now describe the structure of the proof.
+  We want to go from seq_cont F to dialogue_cont F.
+ Right now, we can do the following.*)
+Lemma GBI_GCI_Fail F :
+  seq_cont F ->
+  dialogue_cont F.
 Proof.
-  induction 1 as [v u [n [r Hr]] Hincl Hfun | q v Hnotin _ IHk] ; intros.
-  - have aux := eval_ext_tree_aux_finapp_monotone_output_list Hfun Hincl Hr.
-    clear u Hr Hincl.
-    case (leqP n (size v)).
-    { apply (eval_ext_tree_aux_finapp_monotone_output_fuel (size v - n)) in aux.
-      intros Hinf ; apply subnK in Hinf.
-      rewrite addnC in Hinf ; rewrite Hinf in aux.
-      econstructor ; intros u Hu.
-      destruct Hu as [u i i' o Hfunu Hask Hnone | u i i' o Hfunu Hask Hsome ].
-      1,2: rewrite aux in Hask ; now inversion Hask.
-    }
-    intros Hinf ; apply leqW in Hinf ; cbn in Hinf ; apply subnK in Hinf.
-    rewrite addnC in Hinf ; rewrite - Hinf in aux.
-    clear Hinf ; revert r Hfun aux.
-    generalize (n - size v) as k ; intros k ; clear n ; revert v.
-    induction k as [ | k IHk].
-    + intros.
-      rewrite addn0 in aux.
-      econstructor ; intros u Hu.
-      destruct Hu as [ u i i' o Hfunu Hask Hnone | u i i' o Hfunu Hask Hsome ].
-      1,2 : rewrite aux in Hask ; now inversion Hask.
-    + intros.
-      econstructor ; intros u Hu.
-      destruct Hu as [u i i' o Hfunu Hask Hnone | u i i' o Hfunu Hask Hsome ].
-      * apply (IHk _ r) ; [now apply eval_list_none_fun | ].
-        rewrite size_cat addn1 addSn - addnS.
-        unshelve eapply (eval_ext_tree_aux_finapp_monotone_output_list _ _ aux).
-        -- now apply eval_list_none_fun.
-        -- now apply List.incl_appl, List.incl_refl.
-      * apply (IHk _ r) ; [ now apply eval_list_In_is_fun | ].
-        rewrite size_cat addn1 addSn - addnS.
-        unshelve eapply (eval_ext_tree_aux_finapp_monotone_output_list _ _ aux).
-        -- now apply eval_list_In_is_fun.
-        -- now apply List.incl_appl, List.incl_refl.
-  - econstructor ; intros u Hu.
-    destruct Hu as [u i i' o Hfunu Hask Hnone | u i i' o Hfunu Hask Hsome ].
+  intros HF.
+  apply seq_cont_to_seq_cont_valid in HF.
+  destruct HF as [tau [HF Hval]].
+  eapply Delta0_choice in HF as [HF].
+  2:{ intros α n.
+      destruct eval_ext_tree eqn:E.
+      - firstorder congruence.
+      - left. destruct (HF α) as [m].
+        f_equal. 
+        eapply eval_ext_tree_output_unique; eauto. 
+  }
+  pose (T:= fun (l : seq (I * O)) =>
+              exists n a, eval_ext_tree_aux_finapp tau l n nil = output a).
+  have Help : ABbarred T.
+  { intros alpha.
+    destruct (HF alpha) as [n Hn].
+    exists (eval_ext_tree_trace tau alpha n).
+    unfold T.
+    exists n, (F alpha).
+    now eapply eval_ext_tree_finapp_trace.
+  }
+  apply HGBI in Help.
+    (*What we lack is a way to go from indbarred T [::] to dialogue_cont F.*)
 Abort.
+
+(*
+  Going from indbarred T [::] to the existence of a suitable dialogue tree is not easy.
+  We will do so through several
+ intermediate steps :
+ - We will first define a predicate 
+      ext_tree_indbarred : ext_tree -> seq (I * O)) -> Type 
+   such that ext_tree_indbarred tau nil implies
+   {d : dialogue & forall alpha, exists n,
+        eval_ext_tree tau alpha n = output (deval d alpha)}.
+   This will allow us to go from extensional trees to dialogue trees;
+
+ - We will then define a predicate 
+      ext_tree_indbarredP : ext_tree -> seq (I * O) -> Prop
+   tailored to go through singleton elimination.
+   We will then prove that 
+      ext_tree_indbarredP tau l -> ext_tree_indbarred tau l,
+   thus going from Prop to Type.
+
+ - We will then define
+      indbarred_fun_list : (seq (I * O) -> Prop) -> seq (I * O) -> Prop,
+   a variant of indbarred where u : seq (I * O) is a finite approximation 
+   of a function, and prove that
+      indbarred_fun_list (fun l => exists n a,
+                                  eval_ext_tree_aux_finapp tau l n nil = output a) ->
+        ext_tree_indbarredP tau l.
+   This is the longest proof of the file.
+ - Finally, we prove that for any predicate T,
+   indbarred T [::] -> indbarred_fun_list T [::].
+*)
+
+
+(*As explained, let us start by ext_tree_indbarred. 
+  It is an inductive predicate that describes a tree of computations
+  using tau and l, such that on the leaves of the tree
+  eval_ext_tree_aux_finapp tau l (size l) nil = output r
+  for some r.
+  There are three cases for this inductive :
+  - ext_tree_eta is the leaf case, where the computation reaches an output r.
+  - ext_tree_succ deals with the case when the computation is blocked
+    because of the lack of fuel. As we use (size l) as fuel, the way out is
+    simply to make l longer, by extending it with some values (q, a) that
+    are already present in the list. Thus l ++ [::(q, a)] is longer than l
+    but it does not contain more values from a set perspective.
+  - finally, ext_tree_beta deals with the case when the computation is blocked
+    because l does not contain the answer to some query q. In that case, we
+    branch over every possible answer a : A with l ++ [::(q, a)].
+*)
+Inductive ext_tree_indbarred (tau : ext_tree) (l : seq (I * O)) (n : nat) : Type :=
+| ext_tree_eta r : is_fun_list l ->
+                   eval_ext_tree_aux_finapp tau l n nil = output r ->
+                   ext_tree_indbarred tau l n
+| ext_tree_succ q a : is_fun_list l ->
+                      eval_ext_tree_aux_finapp tau l n nil = ask q ->
+                      eval_list l q = Some a ->
+                      ext_tree_indbarred tau l n.+1 ->
+                      ext_tree_indbarred tau l n
+| ext_tree_beta q : is_fun_list l ->
+                    eval_ext_tree_aux_finapp tau l n nil = ask q ->
+                    eval_list l q = None ->
+                    (forall a, ext_tree_indbarred tau (l ++ [:: (q,a)]) n) ->
+                      ext_tree_indbarred tau l n.
+
+
+(*ext_tree_indbarred tau l indeed allows us to retrieve a dialogue tree d.
+ We first prove an auxiliary lemma for any l.*)
+
+Lemma ext_tree_indbarred_dialogue_aux
+  (tau : ext_tree) (Hvalid : valid_ext_tree tau)
+  (l : list (I * O)) (n : nat)
+  (Hyp : ext_tree_indbarred tau l n) :
+  {d : dialogue & forall alpha,
+        l = map (fun i => (i, alpha i)) (map fst l) ->
+        exists n, eval_ext_tree tau alpha n = output (deval d alpha)}.
+Proof.
+  induction Hyp as [l n r Hfun Heval | l n i o Hfun Hask Hsome k [d IHd] |
+                     l n i Hfun Hask Hnone k IHk].
+  - exists (eta r).
+    intros alpha Heqalpha ; exists n ; cbn in *.
+    suff: forall u n l, eval_ext_tree_aux_finapp tau [seq (i, alpha i) | i <- u] n l = output r ->
+                        eval_ext_tree_aux tau alpha n l = output r.
+    { intros Hyp.
+      eapply Hyp with (map fst l) ; cbn.
+      now rewrite - Heqalpha.
+    }
+    clear ; intros.
+    revert l H ; induction n ; cbn ; intros ; [assumption | ].
+    remember (tau l) as aux ; destruct aux as [q | a] ; [ | assumption ].
+    remember (eval_list [seq (i, alpha i) | i <- u] q) as aux2 ; destruct aux2 as [o | ].
+    + eapply IHn.
+      suff: o = alpha q by (intros Heq ; subst ; assumption).
+      eapply eval_list_map_In ; eauto.
+    + now inversion H.
+  - exists d ; intros alpha Heqalpha.
+    now apply (IHd alpha) ; clear IHd.
+  - exists (beta i (fun o => projT1 (IHk o))).
+    intros alpha Heqalpha ; cbn in *.
+    eapply (projT2 (IHk (alpha i))).
+    do 2 rewrite map_cat ; now rewrite - Heqalpha.
+Qed.    
+    
+(*We can then prove our desired lemma when l = nil.*)    
+    
+Lemma ext_tree_indbarred_dialogue
+  (tau : ext_tree) (Hvalid : valid_ext_tree tau) (n : nat)
+  (Hyp : ext_tree_indbarred tau nil n) :
+  {d : dialogue & forall alpha, exists n,
+        eval_ext_tree tau alpha n = output (deval d alpha)}.
+Proof.
+  eapply ext_tree_indbarred_dialogue_aux in Hyp as [d Hd] ; auto.
+  exists d.
+  intros alpha ; eapply Hd ; reflexivity.
+Qed.
+
+
+(*We now define ext_tree_indbarredP, the same predicate as
+ ext_tree_indbarred, albeit living in Prop.
+ We tailor it to go through subsingleton elimination.*)
 
 Unset Elimination Schemes.
 
-Inductive ext_tree_indbarredP (tau : ext_tree) (l: seq (I * O)) : Prop :=
+Inductive ext_tree_indbarredP (tau : ext_tree) (l: seq (I * O)) (n : nat) : Prop :=
 | etree_in : is_fun_list l ->
-             ((exists q, eval_ext_tree_aux_finapp tau l (size l) nil = ask q /\
+             ((exists q, eval_ext_tree_aux_finapp tau l n nil = ask q /\
                            eval_list l q = None /\
-                           (forall a, ext_tree_indbarredP tau (l ++ [:: (q,a)]))) \/
+                           (forall a, ext_tree_indbarredP tau (l ++ [:: (q,a)]) n)) \/
                 
-                (exists r, eval_ext_tree_aux_finapp tau l (size l) nil = output r) \/
+                (exists r, eval_ext_tree_aux_finapp tau l n nil = output r) \/
                 
-                (exists q a, eval_ext_tree_aux_finapp tau l (size l) nil = ask q /\
+                (exists q a, eval_ext_tree_aux_finapp tau l n nil = ask q /\
                              eval_list l q = Some a /\
-                             ext_tree_indbarredP tau (l ++ [:: (q, a)]))) ->
-             ext_tree_indbarredP tau l.
+                             ext_tree_indbarredP tau l n.+1)) ->
+             ext_tree_indbarredP tau l n.
 
 Set Elimination Schemes.
 
-Inductive ext_tree_indbarred (tau : ext_tree) (l : seq (I * O)) : Type :=
-| ext_tree_eta r : is_fun_list l ->
-                   eval_ext_tree_aux_finapp tau l (size l) nil = output r ->
-                   ext_tree_indbarred tau l
-| ext_tree_succ q a : is_fun_list l ->
-                      eval_ext_tree_aux_finapp tau l (size l) nil = ask q ->
-                      eval_list l q = Some a ->
-                      ext_tree_indbarred tau (l ++ [:: (q, a)]) ->
-                      ext_tree_indbarred tau l
-| ext_tree_beta q : is_fun_list l ->
-                    eval_ext_tree_aux_finapp tau l (size l) nil = ask q ->
-                    eval_list l q = None ->
-                    (forall a, ext_tree_indbarred tau (l ++ [:: (q,a)])) ->
-                      ext_tree_indbarred tau l.
-
-(* econstructor ; [assumption | ].
-    right ; left ; exists r.
-    eapply eval_ext_tree_aux_finapp_monotone_output_list ; now eauto.
-  - econstructor ; [assumption | ].
-    right ; right.
-    exists q, a ; split ; [ | split ; [eapply eval_list_monotone ; eassumption | ] ].
-    2:{ eapply ext_tree_indbarredP_monotone_list ; now eauto. }
-    eapply eval_ext_tree_aux_finapp_monotone_ask_list_nomorefuel ; now eauto.
-Defined.    *)
+(*ext_tree_indbarredP can be eliminated into Type.*)
 
 Fixpoint ext_tree_indbarredP_rect
   (tau : ext_tree)
-  (P : seq (I * O) -> Type)
-  (Hout : forall (l : seq (I * O)) (r : A) (Hfun : is_fun_list l)
-                 (e : eval_ext_tree_aux_finapp tau l (size l) [::] = output r), 
-      P l)
-  (Hsucc : forall (l : seq (I * O)) (q : I) (a : O) (Hfun : is_fun_list l)
-                 (Heq : eval_ext_tree_aux_finapp tau l (size l) [::] = ask q)
+  (P : seq (I * O) -> nat -> Type)
+  (Hout : forall (l : seq (I * O)) (n : nat) (r : A) (Hfun : is_fun_list l)
+                 (e : eval_ext_tree_aux_finapp tau l n [::] = output r), 
+      P l n)
+  (Hsucc : forall (l : seq (I * O)) (n : nat) (q : I) (a : O) (Hfun : is_fun_list l)
+                 (Heq : eval_ext_tree_aux_finapp tau l n [::] = ask q)
                  (Hnone : eval_list l q = Some a)
-                 (e : ext_tree_indbarredP tau (l ++ [:: (q, a)])),
-      P (l ++ [:: (q,a) ]) -> P l)
-  (Hask : forall (l : seq (I * O)) (q : I) (Hfun : is_fun_list l)
-                 (Heq : eval_ext_tree_aux_finapp tau l (size l) [::] = ask q)
+                 (e : ext_tree_indbarredP tau l n.+1),
+      P l n.+1 -> P l n)
+  (Hask : forall (l : seq (I * O)) (n : nat) (q : I) (Hfun : is_fun_list l)
+                 (Heq : eval_ext_tree_aux_finapp tau l n [::] = ask q)
                  (Hnone : eval_list l q = None)
-                 (e : forall a : O, ext_tree_indbarredP tau (l ++ [:: (q,a)])),
-      (forall a : O, P (l ++ [:: (q,a)])) -> P l)
-  (l : seq (I * O)) (e : ext_tree_indbarredP tau l) : P l.
+                 (e : forall a : O, ext_tree_indbarredP tau (l ++ [:: (q,a)]) n),
+      (forall a : O, P (l ++ [:: (q,a)]) n) -> P l n)
+  (l : seq (I * O)) (n : nat) (e : ext_tree_indbarredP tau l n) : P l n.
 Proof.
   destruct e as [Hnodup Hq].
-  remember (eval_ext_tree_aux_finapp tau l (size l) [::]) as aux.
+  remember (eval_ext_tree_aux_finapp tau l n [::]) as aux.
   destruct aux as [q | r].
   - remember (eval_list l q) as aux2 ; destruct aux2 as [a | ].
-    + suff: ext_tree_indbarredP tau (l ++ [:: (q, a)]).
+    + suff: ext_tree_indbarredP tau l n.+1.
       { intros Hyp ; eapply Hsucc ; eauto. 
         now apply (ext_tree_indbarredP_rect tau P Hout Hsucc Hask).
       }
-      destruct Hq as [[q' [Heq [Hnone Hq']]] | [[r Hr] | [q' [a' [Heq' [Hq' IH]]]]]] ; [ | now inversion Hr |  ].
+      destruct Hq as [[q' [Heq [Hnone Hq']]] | [[r Hr] | [q' [a' [Heq' [Hq' IH]]]]]] ;
+        [ | now inversion Hr |  ].
       * injection Heq ; intros Heqq ; subst.
         rewrite Hnone in Heqaux2 ; now inversion Heqaux2.
       * inversion Heq' ; subst.
         rewrite Hq' in Heqaux2 ; inversion Heqaux2 ; now subst.
-    + suff: forall a : O, ext_tree_indbarredP tau (l ++ [:: (q, a)]).
+    + suff: forall a : O, ext_tree_indbarredP tau (l ++ [:: (q, a)]) n.
       { intros Hyp.
-        eapply (Hask l q Hnodup) ; [now auto | now symmetry | assumption | ] ; intros a.
+        eapply (Hask l n q Hnodup) ; [now auto | now symmetry | assumption | ] ; intros a.
         apply (ext_tree_indbarredP_rect tau P Hout Hsucc Hask) ; now apply Hyp.
       }
-      destruct Hq as [[q' [Heq' Ho]]| [[r Hr] | [q' [a' [Heval [Hsome Hsuc]]]]]] ; [| now inversion Hr | ].
+      destruct Hq as [[q' [Heq' Ho]]| [[r Hr] | [q' [a' [Heval [Hsome Hsuc]]]]]] ;
+        [| now inversion Hr | ].
       * inversion Heq' ; subst ; now eapply Ho.
       * exfalso.
         injection Heval ; intros Heq ; subst.
         rewrite Hsome in Heqaux2 ; now inversion Heqaux2.
-  - eapply (Hout l r Hnodup).
+  - eapply (Hout l n r Hnodup).
     destruct Hq as [[q [Heq Ho]]| [[r' Hr] | [q' [a' [Heval _]]]]] ; [ now inversion Heq | | now inversion Heval ].
     inversion Hr ; now subst.
 Defined.
@@ -1068,53 +1126,30 @@ Defined.
 
 Lemma ext_tree_indbarredP_ind
   (tau : ext_tree)
-  (P : seq (I * O) -> Prop)
-  (Hout : forall (l : seq (I * O)) (r : A) (Hfun : is_fun_list l)
-                 (e : eval_ext_tree_aux_finapp tau l (size l) [::] = output r), 
-      P l)
-  (Hsucc : forall (l : seq (I * O)) (q : I) (a : O) (Hfun : is_fun_list l)
-                 (Heq : eval_ext_tree_aux_finapp tau l (size l) [::] = ask q)
+  (P : seq (I * O) -> nat -> Prop)
+  (Hout : forall (l : seq (I * O)) (n : nat) (r : A) (Hfun : is_fun_list l)
+                 (e : eval_ext_tree_aux_finapp tau l n [::] = output r), 
+      P l n)
+  (Hsucc : forall (l : seq (I * O)) (n : nat) (q : I) (a : O) (Hfun : is_fun_list l)
+                 (Heq : eval_ext_tree_aux_finapp tau l n [::] = ask q)
                  (Hnone : eval_list l q = Some a)
-                 (e : ext_tree_indbarredP tau (l ++ [:: (q, a)])),
-      P (l ++ [:: (q,a) ]) -> P l)
-  (Hask : forall (l : seq (I * O)) (q : I) (Hfun : is_fun_list l)
-                 (Heq : eval_ext_tree_aux_finapp tau l (size l) [::] = ask q)
+                 (e : ext_tree_indbarredP tau l n.+1),
+      P l n.+1 -> P l n)
+  (Hask : forall (l : seq (I * O)) (n : nat) (q : I) (Hfun : is_fun_list l)
+                 (Heq : eval_ext_tree_aux_finapp tau l n [::] = ask q)
                  (Hnone : eval_list l q = None)
-                 (e : forall a : O, ext_tree_indbarredP tau (l ++ [:: (q,a)])),
-      (forall a : O, P (l ++ [:: (q,a)])) -> P l)
-  (l : seq (I * O)) (e : ext_tree_indbarredP tau l) : P l.
+                 (e : forall a : O, ext_tree_indbarredP tau (l ++ [:: (q,a)]) n),
+      (forall a : O, P (l ++ [:: (q,a)]) n) -> P l n)
+  (l : seq (I * O)) (n : nat) (e : ext_tree_indbarredP tau l n) : P l n.
 Proof.
   eapply ext_tree_indbarredP_rect ; eauto.
 Qed.  
 
 
-
-(*
-  (tau : ext_tree)
-  (P : forall l : seq (I * O), Type)
-       (Hyp : forall (l : seq (I * O)) (q : I) (n : List.NoDup [seq i.1 | i <- l])
-          (e : eval_ext_tree_aux_finapp tau l (size l) [::] = ask q)
-          (e0 : forall a : O, ext_tree_indbarredP tau ((q, a) :: l)),
-        (forall a : O, P ((q, a) :: l)) -> P l)
-        (l : seq (I * O)) (e : ext_tree_indbarredP tau l) : P l.
-Proof.
-  destruct e as [Hnodup Hq].
-  remember (eval_ext_tree_aux_finapp tau l (size l) [::]) as aux.
-  destruct aux as [q | r].
-  - eapply (Hyp l q Hnodup) ; [now auto | | ] ; intros a.
-    + destruct Hq as [q' [Heq' Ho]] ; inversion Heq' ; subst.
-      now eapply Ho.
-    + apply (ext_tree_indbarredP_rect tau P Hyp).
-      destruct Hq as [q' [Heq' Ho]] ; inversion Heq' ; subst.
-      now apply Ho.
-  - exfalso.
-    destruct Hq as [q' [Heq' Ho]].
-    now inversion Heq'.
-Defined.
-*)
+(*ext_tree_indbarredP indeed implies ext_tree_indbarred.*)
 Lemma ext_tree_indbarred_spec (tau : ext_tree) (l : seq (I * O)) (n : nat) :
-  ext_tree_indbarredP tau l ->
-  ext_tree_indbarred tau l.
+  ext_tree_indbarredP tau l n ->
+  ext_tree_indbarred tau l n.
 Proof.
   induction 1 as [l a Hnodup Heqa | l q Hnodup Heq ? IHk  | Hsuc].
   - econstructor 1 ; eassumption.
@@ -1122,92 +1157,294 @@ Proof.
   - econstructor 3 ; now eauto.
 Qed.
 
-Lemma ext_tree_indbarred_dialogue
-  (tau : ext_tree) (Hvalid : valid_ext_tree tau)
-  (Hyp : ext_tree_indbarred tau nil) :
-  {d : dialogue & forall alpha, exists n, eval_ext_tree tau alpha n = output (deval d alpha)}.
-Proof.
-  unfold eval_ext_tree.
-  revert Hyp ; generalize (@nil (I * O)).
-  intros l Hyp ; pattern l.
-  induction Hyp.
-  - exists (eta r).
-    intros alpha ; exists (size l).
-    cbn in *.
-    admit.
-  - assumption.
-  - destruct l as [ | [q' o'] v].
-    + cbn in *.
-      exists (beta q (fun o => projT1 (X o))).
-      intros alpha.
-      destruct (projT2 (X (alpha q)) alpha) as [n Hn].
-      exists n.
-      now cbn.
-    + exact (X o').
-Admitted
-              .
-(*Lemma indbarred_NoDup_NoDup T l:
-  indbarred_NoDup T l ->
-  List.NoDup (map fst l).
-Proof.
-  induction 1 as [ | q v Hnotin k IHk] ; [ assumption | ].
-  destruct v as [ | [q' a] v] ; [now econstructor | ].
-  specialize (IHk a).
-  rewrite map_cat in IHk.
-  now apply List.NoDup_remove_1 in IHk ; rewrite -> cats0 in IHk.
-Qed.
- *)
+
+(*We will now try to go from indbarred to ext_tree_indbarred.
+ We need some technical lemmas for this.*)
+
+(*If eval_ext_tree_aux_finapp tau u n nil = output r,
+ then ext_tree_indbarredP tau u.
+ The idea is that we can add elements (q, a) to u as many times as we need
+ until size u >= n and retrieve
+ eval_ext_tree_aux_finapp tau u (size u) nil = output r
+*)
 
 Lemma eval_output_indbarredP tau u n r :
   is_fun_list u ->
   eval_ext_tree_aux_finapp tau u n nil = output r ->
-  ext_tree_indbarredP tau u.
+  ext_tree_indbarredP tau u n.
 Proof.
   intros Hfun Hyp.
-  case: (leqP n (size u)) ; intros Hinf.
-  - apply subnKC in Hinf.
-    econstructor ; [assumption | right ; left ].
-    exists r ; rewrite - Hinf.
-    now apply eval_ext_tree_aux_finapp_monotone_output_fuel.
-  - apply leqW in Hinf ; cbn in Hinf ; apply subnKC in Hinf.
-    remember (eval_ext_tree_aux_finapp tau u (size u) [::]) as aux ; destruct aux as [q | r'].
-    2: econstructor ; [assumption | right ; left ; now exists r'].
-    remember (eval_list u q) as aux2 ; destruct aux2 as [ a | ].
-    2:{ symmetry in Heqaux ; eapply (eval_ext_tree_aux_finapp_monotone_ask_fuel (n - size u)) in Heqaux ; eauto.
-        rewrite Hinf Hyp in Heqaux ; now inversion Heqaux.
-    }
-    remember (n - size u) as m ; clear Heqm.
-    revert n q a u Hfun Hyp Hinf Heqaux Heqaux2 ; induction m as [ | k IHk] ; intros.
-    + erewrite <- plus_n_O in Hinf ; subst ; exfalso.
-      rewrite Hyp in Heqaux ; now inversion Heqaux.
-    + econstructor ; [assumption | ].
-      right ; right.
-      exists q,a ; split ; [now auto | split ; [now auto | ] ].
-      remember (eval_ext_tree_aux_finapp tau (u ++ [:: (q, a)]) (size u + 1) [::]) as aux3.
-      destruct aux3 as [q' | r'].
-      2:{ econstructor ; [ now apply eval_list_In_is_fun | ].
-          right ; left ; exists r' ; now rewrite size_cat. }
-      remember (eval_list u q') as aux4.
-      destruct aux4 as [a' | ].
-      { apply (IHk n q' a') ; eauto.
-        * now apply eval_list_In_is_fun.
-        * eapply eval_ext_tree_aux_finapp_monotone_output_list ;
-            [ now apply eval_list_In_is_fun | | eassumption ].
-          now apply List.incl_appl, List.incl_refl.
-        * now rewrite <- Hinf, size_cat, <- plus_n_Sm, addn1, plus_Sn_m.
-        * now rewrite size_cat.
-        * symmetry ; eapply eval_list_monotone ; eauto ; [ now apply eval_list_In_is_fun | ].
-          now apply List.incl_appl, List.incl_refl.
-      }
-      exfalso.
-      rewrite <- Hinf, <- plus_n_Sm, <- plus_Sn_m in Hyp.
-      erewrite eval_ext_tree_aux_finapp_monotone_ask_fuel in Hyp ; eauto ; [now inversion Hyp | ].
-      eapply eval_ext_tree_aux_finapp_monotone_ask_list ; eauto ; [ | now rewrite Heqaux3 addn1].
-      apply List.incl_app ; [now apply List.incl_refl | ].
-      intros [x y] [Hin | Hfalse] ; [ inversion Hin ; subst | now eauto].
-      now apply eval_list_In.
-Qed.      
+  econstructor ; [assumption | right ; left ].
+  now exists r.
+Qed.
 
+
+
+(*ext_tree_indbarredP is monotone with respect to list inclusion.
+ This is an intuitive property, the technical part comes from the fact
+ that we use (size u) as fuel, and List.incl u v does not imply
+ size u <= size v, so some care has to be taken.*)
+Lemma ext_tree_indbarredP_monotone tau u v n
+  (Hu : ext_tree_indbarredP tau u n) :
+  is_fun_list v ->
+  List.incl u v ->
+  ext_tree_indbarredP tau v n.
+Proof.
+  revert v ; induction Hu as [u n a Hnodup Heqa | u n q o' Hfunu Heq Hsome _ IHk |
+                               u n q Hfunu Heq Hnoneu _ IHk] ; intros v Hfunv Hincl.
+  - eapply eval_output_indbarredP ; [eassumption | ].
+    eapply eval_ext_tree_aux_finapp_monotone_output_list ; eassumption.
+  - econstructor ; [assumption | right ; right].
+    exists q, o' ; split ; [ | split].
+    + now eapply eval_ext_tree_aux_finapp_monotone_ask_list_nomorefuel ; eauto.
+    + now eapply eval_list_monotone ; eauto.
+    + now apply IHk.
+  - remember (eval_list v q) as aux ; destruct aux as [ a | ].
+    + apply (IHk a _ Hfunv).
+      apply List.incl_app ; [assumption | ].
+      intros [q' o'] [Hyp | Hyp] ; inversion Hyp; subst.
+      now apply eval_list_In.
+    + econstructor ; [assumption | ].
+      left ; exists q ; split ; [ | split ; [now auto | ] ].
+      2: intros a ; apply (IHk a) ; [now apply eval_list_none_fun | auto].
+      * eapply eval_ext_tree_aux_finapp_monotone_ask_list ; now eauto.
+      *  apply List.incl_app ; [ now apply List.incl_appl | ].
+         now apply List.incl_appr, List.incl_refl.
+Qed.
+
+
+Lemma ext_tree_indbarredP_change_fuel tau u n m
+  (Hu : ext_tree_indbarredP tau u n) :
+  ext_tree_indbarredP tau u m.
+Proof.
+  revert m ; induction Hu as [u n a Hnodup Heqa | u n q o Hfunu Heq Hsome _ IHu |
+                               u n q Hfunu Heq Hnoneu _ IHu] ; intros m.
+  - econstructor ; [ assumption | ].
+    case: (leqP n m) ; intros Hinf ; [ | apply leqW in Hinf ; cbn in Hinf] ;
+      apply subnKC in Hinf.
+    + rewrite - Hinf; right ; left ; exists a.
+      now eapply eval_ext_tree_aux_finapp_monotone_output_fuel.
+    + revert Hinf ; generalize (n - m) as k.
+      intros k; revert m n Heqa ; induction k ; intros m n Heqa Hinf.
+      * rewrite addn0 in Hinf ; subst.
+        eauto.
+      * remember (eval_ext_tree_aux_finapp tau u m [::]) as aux.
+        destruct aux as [q | r] ; [ | now eauto].
+        right ; right.
+        remember (eval_list u q) as aux2 ; destruct aux2 as [o | ].
+        -- exists q, o ; split ; [auto | split ; [auto | ] ].
+           econstructor ; [ assumption | ].
+           specialize (IHk m.+1).
+           eapply IHk ; [eauto | ].
+           now rewrite addSn - addnS.
+        -- symmetry in Heqaux ; rewrite - Hinf in Heqa.
+           erewrite eval_ext_tree_aux_finapp_monotone_ask_fuel in Heqa ; eauto.
+           now inversion Heqa.
+  - now eapply IHu.
+  - econstructor ; [ assumption | ].
+    case: (leqP n m) ; intros Hinf ; [ | apply leqW in Hinf ; cbn in Hinf] ;
+      apply subnKC in Hinf.
+    + rewrite - Hinf; left ; exists q ; split ; [ | split ; eauto].
+      now eapply eval_ext_tree_aux_finapp_monotone_ask_fuel ; eauto.
+    + revert Hinf ; generalize (n - m) as k.
+      intros k; revert m n Heq ; induction k ; intros m n Heq Hinf.
+      * rewrite addn0 in Hinf ; subst ; now eauto.
+      * remember (eval_ext_tree_aux_finapp tau u m [::]) as aux.
+        destruct aux as [q' | r] ; [ | now eauto].
+        remember (eval_list u q') as aux2 ; destruct aux2 as [o | ].
+        -- right ; right ; exists q', o ; split ; [auto | split ; [auto | ] ].
+           econstructor ; [ assumption | ].
+           specialize (IHk m.+1).
+           eapply IHk ; [eauto | ].
+           now rewrite addSn - addnS.
+        -- symmetry in Heqaux ; rewrite - Hinf in Heq.
+           erewrite eval_ext_tree_aux_finapp_monotone_ask_fuel in Heq ; eauto.
+Qed.
+
+
+(*When going from some version of indbarred to ext_tree_indbarred,
+ the difficult part will be dealing with the split case.
+ Indeed, in indbarred splitting can be done on any query q, while
+ in ext_tree_indbarred it has to be done on a query q such that
+ eval_ext_tree_aux_finapp tau u (size u) = ask q.
+ We thus need to reorganise splittings, or even get rid of them 
+ in branches where they are not necessary.
+ To do this, we use the predicate List.Add, to generalize addition
+ of an element to the list u.*)
+
+Lemma Add_induction_step (tau : ext_tree) (u v : seq (I * O)) (n : nat) (i : I) (o : O) :
+  eval_list u i = None ->
+  List.Add (i, o) u v ->
+  (ext_tree_indbarredP tau v n) ->
+  (forall a w, List.Add (i, a) u w ->
+               ext_tree_indbarredP tau w n) ->
+  ext_tree_indbarredP tau u n.
+Proof.
+  intros Hnone Hadd Hv Hyp.
+  have Hincl : List.incl u v.
+  { intros x Hin ; eapply List.Add_in ; [eassumption | now right]. }
+  revert u Hincl Hnone Hadd Hyp.
+  induction Hv as [l n a Hnodup Heqa | l n q o' Hfunl Heq Hsome k IHk |
+                    l n q Hfunl Heq Hnonel k IHk] ; intros.
+  all: have Hfunu : is_fun_list u by (eapply is_fun_list_incl ; eassumption). 
+  - remember (eval_ext_tree_aux_finapp tau u n nil) as aux.
+    destruct aux as [q' | r].
+    2: econstructor ; [ assumption | right ; left ; now exists r].
+    remember (eval_list u q') as aux2 ; destruct aux2 as [a' | ].
+    + econstructor ; [assumption | right ; right ; exists q', a' ].
+      split ; [now auto | split ; [now auto | ] ].
+      symmetry in Heqaux.
+      eapply (eval_ext_tree_aux_finapp_monotone_ask_list_nomorefuel (v := l)) in Heqaux ;
+        eauto.
+      rewrite Heqaux in Heqa ; now inversion Heqa.
+    + destruct (@eqP I q' i) as [Heq' | Hnoteq] ; [subst | ].
+      * econstructor ; [assumption | ].
+        left ; exists i ; split ; [auto | split ; [assumption | ] ].
+        intros a' ; apply (Hyp a').
+        rewrite cats1 ; now apply Add_rcons.
+      * exfalso.
+        suff: eval_ext_tree_aux_finapp tau l n [::] = ask q'.
+        { intros Heq' ; rewrite Heq' in Heqa ; now inversion Heqa. }
+        eapply eval_ext_tree_aux_finapp_monotone_ask_list ; eauto.
+        eapply eval_list_incl_none with (u ++ [:: (i, o)]) ; eauto.
+        -- now apply eval_list_none_fun.
+        -- intros x Hinx.
+           eapply (List.Add_in Hadd) in Hinx.
+           destruct Hinx as [Hl | Hr] ; apply List.in_or_app ; [right | ] ; now left.
+        -- apply eval_list_notin_cat ; [now auto | cbn].
+           intros [Heqi | Hfalse] ; auto.
+  - remember (eval_ext_tree_aux_finapp tau u n nil) as aux.
+    destruct aux as [q' | r].
+    2: econstructor ; [ auto | right ; left ; now exists r ].
+    remember (eval_list u q') as aux2 ; destruct aux2 as [a | ].
+    + econstructor ; [ auto | ].
+      right ; right ; exists q',a.
+      split ; [now auto | split ; [now auto | ] ].
+      eapply IHk ; eauto.
+      intros a' w Haddw ; eapply ext_tree_indbarredP_change_fuel ; eauto.
+    + destruct (@eqP I q' i) as [Heqi | Hnoteq] ; [subst | exfalso ].
+      * econstructor ; [assumption | left].
+        exists i ; split ; [auto | split ; [auto | ] ].
+        intros a ; apply (Hyp a).
+        rewrite cats1 ; now apply Add_rcons.
+      * suff: eval_list l q' = None ; [ intros auxl | ].
+        -- suff: ask (R := A) q = ask q' by
+             (intros H ; inversion H ; subst ; rewrite auxl in Hsome ; inversion Hsome).
+           rewrite - Heq.
+           eapply eval_ext_tree_aux_finapp_monotone_ask_list ; eauto.
+        -- eapply eval_list_incl_none with (u ++ [::(i, o)]).
+           ++ now apply eval_list_none_fun.
+           ++ intros x Hinx ; eapply (List.Add_in Hadd) in Hinx.
+              destruct Hinx as [Hinx | Hinx] ; eapply List.in_or_app ; [| now left].
+              right ; now left.
+           ++ eapply eval_list_notin_cat ; auto ; cbn.
+              intros [Hin | Hin] ; inversion Hin ; now auto.
+  - remember (eval_ext_tree_aux_finapp tau u n nil) as aux.
+    destruct aux as [q' | r].
+    2: econstructor ; [ assumption | right ; left ; now exists r ].
+    remember (eval_list u q') as aux2 ; destruct aux2 as [a | ].
+    + econstructor ; [ assumption | ].
+      right ; right ; exists q',a.
+      split ; [now auto | split ; [now auto | ] ].
+      remember (eval_ext_tree_aux_finapp tau u n.+1 nil) as aux3.
+      destruct aux3 as [q'' | r].
+      2: econstructor ; [ assumption | right ; left ; now exists r ].
+      have Heqq: q'' = q ; [ | subst].
+      { suff: ask (R := A) q'' = ask q by (intros H ; inversion H).
+        eapply (eval_ext_tree_aux_finapp_monotone_ask_fuel 1) in Heq ; eauto.
+        rewrite Heqaux3 - Heq addn1.
+        eapply eval_ext_tree_aux_finapp_one_step_fuel ; eauto.
+      }
+      econstructor ; [assumption | left].
+      exists q ; split ; [auto | split ; [now apply eval_list_incl_none with l | ] ].
+      intros o'.
+      have Hnoneu: eval_list (u ++ [:: (q, o')]) i = None.
+      { apply eval_list_notin_cat ; [assumption | cbn].
+        intros [Heqi | Hfalse] ; [ subst | now inversion Hfalse].
+        suff: eval_list l i = Some o by (intros H ; rewrite Hnonel in H ; now inversion H).
+        apply (In_eval_list Hfunl), (List.Add_in Hadd) ; now left.
+      }
+      eapply ext_tree_indbarredP_change_fuel with n.
+      eapply (IHk o') ; eauto.
+      -- apply List.incl_app ; [now apply List.incl_appl | ].
+         apply List.incl_appr, List.incl_refl.
+      -- now apply Add_cat.
+      -- intros a' w Haddw.
+         eapply ext_tree_indbarredP_monotone with ((i,a') :: u).
+         ** now apply Hyp with a', List.Add_head.
+         ** eapply is_fun_list_incl with ((u ++ [:: (q, o')]) ++ [::(i, a')]).
+            { apply eval_list_none_fun ; auto ; apply eval_list_none_fun ; auto.
+              apply eval_list_incl_none with l ; eauto.
+            }
+            intros y Hiny ; apply (List.Add_in Haddw) in Hiny.
+            destruct Hiny as [Hiny | Hiny] ; [subst | ].
+            --- apply List.in_or_app ; right ; now left.
+            --- apply List.in_or_app ; now left.
+         ** intros x Hinx.
+            eapply (List.Add_in Haddw) ; rewrite - cat_cons.
+            apply List.in_or_app ; now left.
+    + suff: q' = i \/ (q' <> i /\ q' = q) ; [intros [Heqi | [Hnoteq Heqq] ] ; subst | ].
+      * econstructor ; [assumption | ].
+        left ; exists i ; split ; [auto | split ; [ auto | intros o'] ].
+        apply (Hyp o') ; rewrite cats1 ; now apply Add_rcons.
+      * econstructor ; [assumption | ].
+        left ; exists q ; split ; [auto | split ; [ auto | ] ].
+        intros o' ; eapply (IHk o').
+        -- apply List.incl_app ; [now apply List.incl_appl | ].
+           apply List.incl_appr, List.incl_refl.
+        -- apply eval_list_notin_cat ; [assumption | ].
+           cbn ; intros [Heqi | Hfalse] ; subst ; now auto.
+        -- now apply Add_cat.
+        -- intros a w Haddw.
+           eapply ext_tree_indbarredP_monotone with ((i,a) :: u).
+           ++ now apply Hyp with a, List.Add_head.
+           ++ eapply is_fun_list_incl with ((u ++ [:: (q, o')]) ++ [::(i, a)]).
+              { apply eval_list_none_fun ; auto ; [ now apply eval_list_none_fun | ].
+                apply eval_list_notin_cat ; auto ; cbn.
+                intros [Heqi | Hfalse] ; [now subst | now inversion Hfalse].
+              }
+              intros y Hiny ; apply (List.Add_in Haddw) in Hiny.
+              destruct Hiny as [Hiny | Hiny] ; [subst | ].
+              ** apply List.in_or_app ; right ; now left.
+              ** apply List.in_or_app ; now left.
+           ++ intros x Hinx.
+              eapply (List.Add_in Haddw) ; rewrite - cat_cons.
+              apply List.in_or_app ; now left.
+      * destruct (@eqP I q' i) as [ | Hnoteq] ; [now left | right ; split ; auto].
+        suff: ask (R := A) q = ask q' by (inversion 1).
+        erewrite <- Heq ; eauto.
+        eapply eval_ext_tree_aux_finapp_monotone_ask_list ; eauto.
+        eapply eval_list_incl_none with ((i,o) :: u).
+        -- eapply is_fun_cons_notin_dom ; eauto ; now apply eval_list_notin.
+        -- intros x Hinx ; now apply (List.Add_in Hadd) in Hinx.
+        -- cbn ; erewrite ifN_eq ; [now auto | ].
+           now eapply contra_not_neq with (q' = i).
+Qed.
+
+
+Inductive indbarred_fun_list (T : seq (I * O) -> Prop) : seq (I * O) -> Prop :=
+| ieta_fun_list : forall u' u : seq (I * O),
+    T u -> List.incl u u' -> is_fun_list u' -> indbarred_fun_list T u'
+| ibeta_NoDup : forall (a : I) (v : seq (I * O)),
+    ~ List.In a [seq i.1 | i <- v] ->
+    (forall b : O, indbarred_fun_list T (v ++ [:: (a, b)])) ->
+    indbarred_fun_list T v.
+
+
+
+Lemma indbarred_indbarred_fun_list (T : seq (I * O) -> Prop) :
+  indbarred T nil ->
+  indbarred_fun_list T nil.
+Proof.
+  have aux: is_fun_list (@nil (I * O)).
+  { intros q r r' Hin ; now inversion Hin. }
+  revert aux ; generalize (@nil (I * O)) ; intros l Hfun Hyp ; revert Hfun.
+  induction Hyp as [u v Hv Hincl | i v Hnotin k IHk ] ; intros.
+  { econstructor ; eassumption. }
+  econstructor 2 ; [ now apply Hnotin |].
+  intros o ; apply IHk.
+  rewrite cats1 ; apply is_fun_rcons_notin_dom ; assumption.
+Qed.
 
 Lemma indbarred_fun_list_fun_list T l:
   indbarred_fun_list T l ->
@@ -1220,566 +1457,32 @@ Proof.
   now apply List.incl_appl, List.incl_refl.
 Qed.
 
-
-Fixpoint ext_tree_indbarredP_monotone tau u v
-  (Hu : ext_tree_indbarredP tau u) {struct Hu}:
-  is_fun_list v ->
-  List.incl u v ->
-  ext_tree_indbarredP tau v.
-Proof.
-  intros Hfunv Hincl.
-  destruct Hu as [Hfunu Hyp].
-  destruct Hyp as [[q [Heq [Hnone Hq]]]| [[r Hr] | [q [a [Heval [Hsome Hsuc]]]]]].
-  - remember (eval_list v q) as aux ; destruct aux as [ a | ].
-    + apply (ext_tree_indbarredP_monotone tau _ _ (Hq a) Hfunv).
-      apply List.incl_app ; [assumption | ].
-      intros [q' o'] [Hyp | Hyp] ; inversion Hyp; subst.
-      now apply eval_list_In.
-    + suff: forall (a : O) w, List.incl (v ++ [:: (q, a)]) w ->
-                              is_fun_list w ->
-                              ext_tree_indbarredP tau w.
-      2:{ intros a w Hincl' Hfun' ; apply (ext_tree_indbarredP_monotone tau _ _ (Hq a) Hfun').
-          eapply List.incl_tran ; [ | eassumption].
-          apply List.incl_app ; [now apply List.incl_appl | apply List.incl_appr].
-          now apply List.incl_refl.
-      }
-      intros Hyp.
-      case: (leqP (size u) (size v)) ; intros Hinf.
-      * apply subnKC in Hinf.
-        econstructor ; [assumption | ].
-        left ; exists q ; split ; [ | split ; [now auto | ] ].
-        2:{ intros a ; apply (Hyp a) ; [now apply List.incl_refl | ].
-            rewrite cats1 ; apply is_fun_rcons_notin_dom ; [assumption | ].
-            now apply eval_list_notin.
-        }
-        rewrite - Hinf.
-        erewrite (eval_ext_tree_aux_finapp_monotone_ask_fuel (size v - size u)) ; eauto.
-        eapply eval_ext_tree_aux_finapp_monotone_ask_list ; now eauto.
-      * apply leqW in Hinf ; cbn in Hinf ; apply subnKC in Hinf ; rewrite - Hinf in Heq.
-        remember (size u - size v) as n ; clear Heqn.
-        revert u v Hinf Hincl Hfunu Hfunv Hnone Hq Heq Heqaux Hyp.
-        induction n ; cbn ; intros.
-        { rewrite <- plus_n_O in Hinf, Heq.
-          econstructor ; [assumption | ].
-          left ; exists q ; split ;
-            [now eapply eval_ext_tree_aux_finapp_monotone_ask_list ; eauto | ].
-          split ; [now eauto | ].
-          intros a ; apply (Hyp a) ; [now apply List.incl_refl | ].
-          rewrite cats1 ; apply is_fun_rcons_notin_dom ; [assumption | ].
-          now apply eval_list_notin.
-        }
-        remember (eval_ext_tree_aux_finapp tau v (size v) [::]) as auxv ; destruct auxv as [q' | ].
-        2:{ eapply eval_ext_tree_aux_finapp_monotone_ask_list in Heq ; eauto.
-            symmetry in Heqauxv.
-            eapply (eval_ext_tree_aux_finapp_monotone_output_fuel n.+1) in Heqauxv ; eauto.
-            rewrite Heq in Heqauxv ; now inversion Heqauxv.
-        }
-        case: (@eqP I q q') ; [intros Heqq ; subst | intros Hnoteq].
-        -- econstructor ; [assumption | ].
-           left ; exists q' ; split ; [now auto | split ; [now trivial | ]].
-           intros a ; apply (Hyp a) ; [now apply List.incl_refl | ].
-           rewrite cats1 ; apply is_fun_rcons_notin_dom ; [assumption | ].
-           now apply eval_list_notin.
-        -- econstructor ; [assumption | ].
-           remember (eval_list v q') as auxv ; destruct auxv as [ a| ].
-           { right ; right.
-             exists q', a ; split ; [now auto | split ; [now auto | ] ].
-             apply (IHn u) ; eauto.
-             ++ rewrite size_cat ; cbn ; now rewrite -> addn1, plus_Sn_m, plus_n_Sm.
-             ++ now apply List.incl_appl.
-             ++ now apply eval_list_In_is_fun.
-             ++ now rewrite size_cat ; cbn ; rewrite -> addn1, plus_Sn_m, plus_n_Sm.
-             ++ symmetry ; apply eval_list_notin_cat ; [now auto | cbn].
-                intros [Heq' | Hfalse] ; [ subst | now inversion Hfalse].
-                now apply Hnoteq.
-             ++ intros a' w Hincl' Hfunw.
-                apply (Hyp a') ; [ | assumption].
-                eapply List.incl_tran ; [ | eassumption].
-                apply List.incl_app ; [do 2 apply List.incl_appl ; now apply List.incl_refl | ].
-                now apply List.incl_appr, List.incl_refl.
-           }
-           left.
-           exists q' ; split ; [now auto | split ; [now auto | ] ].
-           intros a.
-           eapply (IHn u) ; eauto.
-           ++ rewrite size_cat ; cbn ; now rewrite -> addn1, plus_Sn_m, plus_n_Sm.
-           ++ now apply List.incl_appl.
-           ++ rewrite cats1 ; apply is_fun_rcons_notin_dom ; [assumption | ].
-              now apply eval_list_notin.
-           ++ now rewrite <- Heq, size_cat, <- plus_n_Sm, <- plus_Sn_m, addn1.
-           ++ symmetry ; apply eval_list_notin_cat ; [now auto | cbn].
-              intros [Heq' | Hfalse] ; [ subst | now inversion Hfalse].
-              now apply Hnoteq.
-           ++ intros a' w Hincl' Hfunw.
-              apply (Hyp a') ; [ | assumption].
-              eapply List.incl_tran ; [ | eassumption].
-              apply List.incl_app ; [do 2 apply List.incl_appl ; now apply List.incl_refl | ].
-              now apply List.incl_appr, List.incl_refl.
-  - eapply eval_output_indbarredP ; [eassumption | ].
-    eapply eval_ext_tree_aux_finapp_monotone_output_list ; eassumption.
-  - apply (ext_tree_indbarredP_monotone _ _ _ Hsuc Hfunv).
-    apply List.incl_app ; [assumption | ].
-    intros [x y] [Hin | Hfalse] ; [ inversion Hin ; subst | now inversion Hfalse].
-    now apply Hincl, eval_list_In.
-Defined.    
-
-Print eval_ext_tree_aux_finapp.
-
-Fixpoint eval_ext_tree_aux_finapp_minimal_list
-  (tau : ext_tree (R := A)) (u : seq (I * O)) (n : nat) (l : seq O) {struct n} :
-    seq (I * O) :=
-  match n, tau l with
-  | 0, _ => [::]
-  | _, output _ => [::]
-  | k.+1, ask q => match eval_list u q with
-                   | None => [::]
-                   | Some o => (q, o) :: eval_ext_tree_aux_finapp_minimal_list tau u k (rcons l o)
-                   end
-  end.
-
-Print List.Add.
-
-Lemma Add_rcons {X : Type} (a : X) (l : seq X): List.Add a l (rcons l a).
-Admitted.
-
-Lemma Add_cat {X : Type} (a : X) (u v w : seq X) :
-  List.Add a u v ->
-  List.Add a (u ++ w) (v ++ w).
-Admitted.
-
-Lemma Add_diamond {X : Type} (x y : X) (u v w l : seq X) :
-  List.Add x u v -> List.Add y v l -> List.Add x w l -> List.Add y u w.
-Admitted.
-
-
-Lemma super (tau : ext_tree) (u v : seq (I * O)) (i : I) (o : O) :
-  eval_list u i = None ->
-  List.Add (i,o) u v ->
-  (ext_tree_indbarredP tau v) ->
-  (forall a w, List.Add (i, a) u w ->
-               ext_tree_indbarredP tau w) ->
-  ext_tree_indbarredP tau u.
-Proof.
-  intros Hnone Hadd Hv Hyp.
-  have Hincl : List.incl u v.
-  { intros x Hin ; eapply List.Add_in ; [eassumption | now right]. }
-  revert u Hincl Hnone Hadd Hyp.
-  induction Hv as [l a Hnodup Heqa | l q o' Hfunl Heq Hsome k IHk |
-                    l q Hfunl Heq Hnonel k IHk] ; intros.
-  - have Hfunu : is_fun_list u.
-    { eapply is_fun_list_incl ; eassumption. } 
-    have Heq: (size l = (size u).+1) by (eapply List.Add_length ; eassumption).
-    rewrite Heq in Heqa.
-    remember (eval_ext_tree_aux_finapp tau u (size u) nil) as aux.
-    destruct aux as [q' | r].
-    2: econstructor ; [ assumption | right ; left ; now exists r].
-    remember (eval_list u q') as aux2 ; destruct aux2 as [a' | ].
-    + econstructor ; [assumption | right ; right ; exists q', a' ].
-      split ; [now auto | split ; [now auto | ] ].
-      remember (eval_ext_tree_aux_finapp tau (u ++ [:: (q', a')]) (size u).+1 [::])
-        as aux3.
-      destruct aux3 as [q'' | r'].
-      2:{ econstructor ; [ now apply eval_list_In_is_fun | ].
-          right ; left ; exists r' ; now rewrite size_cat addn1.
-      }
-      econstructor ; [now apply eval_list_In_is_fun | right ; left ].
-      exists a ; rewrite size_cat addn1 - Heqa.
-      eapply (eval_ext_tree_aux_finapp_one_step_fuel) ; eauto.
-      * now apply eval_list_In_is_fun.
-      * now apply List.incl_appl, List.incl_refl.
-    + destruct (@eqP I q' i) as [Heq' | Hnoteq] ; [subst | ].
-      * econstructor ; [assumption | ].
-        left ; exists i ; split ; [auto | split ; [assumption | ] ].
-        intros a' ; apply (Hyp a').
-        rewrite cats1 ; now apply Add_rcons.
-      * exfalso.
-        suff: eval_ext_tree_aux_finapp tau l (size u).+1 [::] = ask q'.
-        {intros Heq' ; rewrite Heq' in Heqa ; now inversion Heqa. }
-        suff: eval_list l q' = None.
-        { intros Hnonel.
-          rewrite - addn1 ; apply eval_ext_tree_aux_finapp_monotone_ask_fuel ; auto .
-          now eapply eval_ext_tree_aux_finapp_monotone_ask_list ; eauto.
-        }
-        suff: eval_list (u ++ [::(i,o)]) q' = None.
-        { intros Hnoneu.
-          eapply eval_list_incl_none with (u ++ [:: (i, o)]) ; eauto.
-          * now apply eval_list_none_fun.
-          * intros x Hinx.
-            eapply (List.Add_in Hadd) in Hinx.
-            destruct Hinx as [Hl | Hr] ; apply List.in_or_app ; [right | ] ; now left.
-        }
-        apply eval_list_notin_cat ; [now auto | cbn].
-        intros [Heqi | Hfalse] ; auto.
-  - have Hfunu : is_fun_list u by (eapply is_fun_list_incl ; eassumption).
-    have Heqsize : size l = (size u).+1 by (eapply List.Add_length ; eassumption).
-    rewrite Heqsize in Heq.
-    remember (eval_ext_tree_aux_finapp tau u (size u) nil) as aux.
-    destruct aux as [q' | r].
-    2: econstructor ; [ auto | right ; left ; now exists r ].
-    remember (eval_list u q') as aux2 ; destruct aux2 as [a | ].
-    + econstructor ; [ auto | ].
-      right ; right ; exists q',a.
-      split ; [now auto | split ; [now auto | ] ].
-      remember (eval_ext_tree_aux_finapp tau (u ++[:: (q', a)]) (size (u ++ [:: (q', a)])) nil)
-        as aux3.
-      destruct aux3 as [q'' | r].
-      2: econstructor ; [ now apply eval_list_In_is_fun | right ; left ; now exists r ].
-      suff: q'' = q.
-      2:{ suff: ask (R:= A) q'' = ask q ; [ intros H ; now inversion H | ].
-          rewrite Heqaux3 - Heq size_cat addn1.
-          erewrite (eval_ext_tree_aux_finapp_one_step_fuel (u := u) (v := l)) ; eauto.
-          * now apply eval_list_In_is_fun.
-          * apply List.incl_appl, List.incl_refl.
-      }
-      intros H ; subst.
-      remember (eval_list u q) as aux4 ; destruct aux4 as [a' | ].
-      * have auxeq : o' = a'.
-        { suff : Some o' = Some a' by (intros H ; now inversion H).
-          rewrite - Hsome ; eapply eval_list_monotone ; eauto.
-        }
-        subst.
-        have auxeval : eval_list (u ++ [:: (q', a)]) q = Some a'.
-        { eapply eval_list_monotone with u ; [now apply eval_list_In_is_fun | | eauto ].
-          now apply List.incl_appl, List.incl_refl.
-        }
-        econstructor ; [now apply eval_list_In_is_fun | right ; right ].
-        exists q, a' ; split ; [auto | split ; [ auto | ] ].
-        suff: ext_tree_indbarredP tau (u ++ [::(q,a')]).
-        { intros H ; apply (ext_tree_indbarredP_monotone H).
-          + apply eval_list_In_is_fun ; [ now apply eval_list_In_is_fun | auto ].
-          + apply List.incl_app ; [ | now apply List.incl_appr, List.incl_refl].
-            do 2 apply List.incl_appl ; now apply List.incl_refl.
-        }
-        destruct (@eqP I i q) as [e | n] ; [ subst | ].
-        { rewrite - Heqaux4 in Hnone ; now inversion Hnone. }
-        unshelve eapply IHk.
-        -- apply List.incl_app ; [now apply List.incl_appl | ].
-           apply List.incl_appr, List.incl_refl.
-        -- apply eval_list_notin_cat ; [assumption | ].
-           cbn ; intros [Hfalse | Hfalse] ; [ | now inversion Hfalse].
-           now apply n.
-        -- now apply Add_cat.
-        -- intros o' w Haddw.
-           suff: ext_tree_indbarredP tau (u ++ [::(i, o')]).
-           { intros H ; unshelve eapply (ext_tree_indbarredP_monotone H).
-             + eapply is_fun_list_incl with ((u ++ [:: (q, a')]) ++ [::(i, o')]).
-               { apply eval_list_none_fun ; [ now apply eval_list_In_is_fun | ].
-                 eapply eval_list_incl_none with u ; eauto.
-                 apply List.incl_app ; [now apply List.incl_refl | ].
-                 apply List.incl_cons ; [ | now apply List.incl_nil_l].
-                 now apply eval_list_In.
-               }
-               intros y Hiny ; apply (List.Add_in Haddw) in Hiny.
-               destruct Hiny as [Hiny | Hiny] ; [subst | ].
-               ++ apply List.in_or_app ; right ; now left.
-               ++ apply List.in_or_app ; now left.
-             + intros x Hin ; eapply List.Add_in ; [eassumption | ].
-               destruct (List.in_app_or _ _ _ Hin) as [Hin2 | Hin2] ; [right | ].
-               * now apply List.in_or_app ; left.
-               * destruct Hin2 as [Hin2 | Hin2] ; inversion Hin2 ; now left.
-           }
-           eapply (Hyp o').
-           rewrite <- cat1s, <- (cats0 u) at 1.
-           apply List.Add_app.
-      * have auxeval : eval_list (u ++ [:: (q', a)]) q = None.
-        { eapply eval_list_incl_none with u ; eauto.
-          apply List.incl_app ; [now apply List.incl_refl | ].
-          intros x [Hinx | Hinx] ; inversion Hinx.
-          now apply eval_list_In.
-        }
-        econstructor ; [ now apply eval_list_In_is_fun | left].
-        exists q ; split ; [ now auto | split ; [ auto | ] ].
-        intros a'.
-        suff: ext_tree_indbarredP tau (u ++ [::(q, a')]).
-        { intros H ; unshelve eapply (ext_tree_indbarredP_monotone H).
-          + rewrite cats1 ; apply is_fun_rcons_notin_dom.
-            * now apply eval_list_In_is_fun.
-            * now apply eval_list_notin.
-          + apply List.incl_app ; [ | now apply List.incl_appr,List.incl_refl].
-            do 2 apply List.incl_appl ; now apply List.incl_refl.
-        }
-        destruct (@eqP I q i) as [Heqi | Hnoteq] ; [subst | exfalso ].
-        -- apply (Hyp a').
-           rewrite cats1 ; now apply Add_rcons.
-        -- suff: eval_list l q = None by (intros H ; rewrite H in Hsome ; now inversion Hsome).
-           eapply eval_list_incl_none with (u ++ [::(i, o)]).
-           ++ now apply eval_list_none_fun.
-           ++ intros x Hinx ; eapply (List.Add_in Hadd) in Hinx.
-              destruct Hinx as [Hinx | Hinx] ; eapply List.in_or_app ; [| now left].
-              right ; now left.
-           ++ eapply eval_list_notin_cat ; auto ; cbn.
-              intros [Hin | Hin] ; inversion Hin ; now auto.
-    + destruct (@eqP I q' i) as [Heqi | Hnoteq] ; [subst | exfalso ].
-      * econstructor ; [assumption | left].
-        exists i ; split ; [auto | split ; [auto | ] ].
-        intros a ; apply (Hyp a).
-        rewrite cats1 ; now apply Add_rcons.
-      * have auxl : eval_list l q' = None.
-        -- eapply eval_list_incl_none with (u ++ [::(i, o)]).
-           ++ now apply eval_list_none_fun.
-           ++ intros x Hinx ; eapply (List.Add_in Hadd) in Hinx.
-              destruct Hinx as [Hinx | Hinx] ; eapply List.in_or_app ; [| now left].
-              right ; now left.
-           ++ eapply eval_list_notin_cat ; auto ; cbn.
-              intros [Hin | Hin] ; inversion Hin ; now auto.
-        -- suff: ask (R := A) q = ask q' by
-             (intros H ; inversion H ; subst ; rewrite auxl in Hsome ; inversion Hsome).
-           rewrite - Heq.
-           eapply eval_ext_tree_aux_finapp_monotone_ask_list ; eauto.
-           rewrite - addn1 ; now apply eval_ext_tree_aux_finapp_monotone_ask_fuel.
-  - have Hfunu : is_fun_list u.
-    { eapply is_fun_list_incl ; eassumption. } 
-    remember (eval_ext_tree_aux_finapp tau u (size u) nil) as aux.
-    destruct aux as [q' | r].
-    2: econstructor ; [ assumption | right ; left ; now exists r ].
-    remember (eval_list u q') as aux2 ; destruct aux2 as [a | ].
-    + econstructor ; [ assumption | ].
-      right ; right ; exists q',a.
-      split ; [now auto | split ; [now auto | ] ].
-      remember (eval_ext_tree_aux_finapp tau (u ++[:: (q', a)]) (size (u ++ [:: (q', a)])) nil)
-        as aux3.
-      destruct aux3 as [q'' | r].
-      2: econstructor ; [now apply eval_list_In_is_fun | right ; left ; now exists r ].
-      suff: q'' = q.
-      2:{ suff: ask (R := A) q'' = ask q by (intros H ; inversion H).
-          have Heqsize: (size l = (size u).+1) by (eapply List.Add_length ; eassumption).
-          rewrite Heqaux3 - Heq size_cat addn1 Heqsize.
-          eapply eval_ext_tree_aux_finapp_one_step_fuel ; eauto.
-          * now apply eval_list_In_is_fun.
-          * now apply List.incl_appl, List.incl_refl.
-      }
-      intros e ; subst.
-      have Hnone': eval_list (u ++ [:: (q', a)]) q = None.
-      { eapply eval_list_incl_none ; [ | | eassumption ] ; auto.
-        eapply List.incl_tran ; [ | exact Hincl].
-        apply List.incl_app ; [now apply List.incl_refl | ].
-        intros x [Hinx | Hinx] ; inversion Hinx ; now apply eval_list_In.
-      }
-      econstructor ; [now apply eval_list_In_is_fun | left].
-      exists q ; split ; [auto | split ; [auto | ] ].
-      intros o'.
-      suff: ext_tree_indbarredP tau (u ++ [::(q, o')]).
-      { intros H ; unshelve eapply (ext_tree_indbarredP_monotone H).
-        + rewrite cats1 ; apply is_fun_rcons_notin_dom.
-          * now apply eval_list_In_is_fun.
-          * now apply eval_list_notin.
-        + apply List.incl_app ; [ | now apply List.incl_appr,List.incl_refl].
-          do 2 apply List.incl_appl ; now apply List.incl_refl.
-      }
-      have Hnoneu: eval_list (u ++ [:: (q, o')]) i = None.
-      { apply eval_list_notin_cat ; [assumption | ].
-        cbn ; intros [Hfalse | Hfalse] ; [ subst | now inversion Hfalse].
-        suff: eval_list l i = Some o.
-        { intros H ; rewrite H in Hnonel ; now inversion Hnonel. }
-        apply (In_eval_list Hfunl).
-        unshelve eapply (List.Add_in Hadd) ; now left.
-      }
-      eapply (IHk o') ; eauto.
-      -- apply List.incl_app ; [now apply List.incl_appl | ].
-         apply List.incl_appr, List.incl_refl.
-      -- now apply Add_cat.
-      -- intros a' w Haddw.
-         suff: exists x, List.Add (q,o') x w.
-         2:{ eapply List.Add_inv.
-             apply (List.Add_in Haddw) ; right ; apply List.in_or_app.
-             right ; now left.
-         }
-         intros [x Haddx].
-         eapply (ext_tree_indbarredP_monotone) with x.
-         ++ eapply Hyp with a'.
-            eapply (@Add_diamond _ _ _ u (u ++ [:: (q, o')]) x w) ; eauto.
-            rewrite cats1 ; eapply Add_rcons.
-         ++ eapply is_fun_list_incl with ((u ++ [:: (q, o')]) ++ [::(i, a')]).
-            { do 2 (apply eval_list_none_fun ; auto).
-              eapply eval_list_incl_none ; [ | | eassumption ] ;
-                [ now apply eval_list_In_is_fun | ].
-              now apply List.incl_appl, List.incl_refl.
-            }
-            intros y Hiny ; apply (List.Add_in Haddw) in Hiny.
-            destruct Hiny as [Hiny | Hiny] ; [subst | ].
-            ** apply List.in_or_app ; right ; now left.
-            ** apply List.in_or_app ; now left.
-         ++ intros y Hin ; eapply List.Add_in ; [eassumption | now right].
-    + destruct (@eqP I q' i) as [Heqi | Hnoteq] ; [ subst | ].
-      * econstructor ; [assumption | ].
-        left ; exists i ; split ; [auto | split ; [ auto | ] ].
-        intros o' ; apply (Hyp o').
-        rewrite cats1 ; now apply Add_rcons.
-      * suff: q' = q ; [intros Heqq ; subst | ].
-        -- econstructor ; [assumption | ].
-           left ; exists q ; split ; [auto | split ; [ auto | ] ].
-           intros o' ; eapply (IHk o').
-           ++ apply List.incl_app ; [now apply List.incl_appl | ].
-              apply List.incl_appr, List.incl_refl.
-           ++ apply eval_list_notin_cat ; [assumption | ].
-              cbn ; intros [Heqi | Hfalse] ; now auto.
-           ++ now apply Add_cat.
-           ++ intros a w Haddw.
-              eapply ext_tree_indbarredP_monotone with ((i,a) :: u).
-              ** now apply Hyp with a, List.Add_head.
-              ** eapply is_fun_list_incl with ((u ++ [:: (q, o')]) ++ [::(i, a)]).
-                 { apply eval_list_none_fun ; auto ; [ now apply eval_list_none_fun | ].
-                   apply eval_list_notin_cat ; auto ; cbn.
-                   intros [Heqi | Hfalse] ; [now subst | now inversion Hfalse].
-                 }
-                 intros y Hiny ; apply (List.Add_in Haddw) in Hiny.
-                 destruct Hiny as [Hiny | Hiny] ; [subst | ].
-                 --- apply List.in_or_app ; right ; now left.
-                 --- apply List.in_or_app ; now left.
-              ** intros x Hinx.
-                 eapply (List.Add_in Haddw) ; rewrite - cat_cons.
-                 apply List.in_or_app ; now left.
-        -- suff: ask (R := A) q = ask q' by (inversion 1).
-           erewrite <- Heq, List.Add_length ; eauto.
-           eapply eval_ext_tree_aux_finapp_monotone_ask_list ; eauto.
-           ++ eapply eval_list_incl_none with ((i,o) :: u).
-              ** eapply is_fun_cons_notin_dom ; eauto.
-                 now apply eval_list_notin.
-              ** intros x Hinx ; now apply (List.Add_in Hadd) in Hinx.
-              ** cbn ; erewrite ifN_eq ; [now auto | ].
-                 eapply contra_not_neq with (q' = i) ; auto.
-           ++ rewrite - addn1.
-              eapply eval_ext_tree_aux_finapp_monotone_ask_fuel ; eauto.
-Qed.
-
-(*              apply eval_list_In_is_fun ; auto.
-              | ].
-              intros y Hiny ; apply (List.Add_in Haddw) in Hiny.
-              destruct Hiny as [Heqy | Hinu] ; [subst | ].
-              
-           admit.
-      * admit.
-    + suff: q' = i.
-      * intros e ; subst.
-        
-      *
-           apply List.Add_split in Haddw as [w1 [w2 [Heqw1 Heqw2]]] ; subst.
-           suff: ext_tree_indbarredP tau (w1 ++ ((i, a') :: w2)%SEQ)
-           
-           remember (eval_list u i) as test ; destruct test as [a' | ].
-           
-           admit.
-        -- 
-        
-
-        -- suff: o' = o.
-           { intros H ; subst.
-             econstructor ; [admit | ].
-             left.
-             exists q ; split ; [auto | split ; [ auto | ] ].
-             intros o'.
-             suff: ext_tree_indbarredP tau (u ++ [::(q, o')]).
-             { intros H ; unshelve eapply (ext_tree_indbarredP_monotone H).
-               + admit.
-               + apply List.incl_app ; [ | now apply List.incl_appr,List.incl_refl].
-                 do 2 apply List.incl_appl ; now apply List.incl_refl.
-             }
-             apply (Hyp o') ; admit.
-           }
-           suff: List.In (q,o) l.
-           { intros H ; apply (In_eval_list Hfunl) in H ; rewrite H in Hsome.
-             now injection Hsome.
-           }
-           eapply List.Add_in ; [exact Hadd | now left].
-        -- econstructor ; [ admit | left].
-           exists q ; split ; [ now auto | split ; [now auto | ] ].
-           intros a'.
-           suff: 
-           cbn.
-           
-           
-             eapply IHk.
-           
-         2:{
-        
-        
-        
-      * suff: q = q''.
-        { intros Heq' ; subst.
-          specialize (IHk i o u (v ++ [::(q'', o')])).
-          Print List.Add.
-          suff: ext_tree_indbarred
-  - subst.
-    econstructor ; [assumption | ].
-    remember (eval_ext_tree_aux_finapp tau u (size u) [::]) as val.
-    destruct val as [q | r].
-    2:{ right ; left ; eauto. }
-    remember (eval_list u q) as val2 ; destruct val2 as [o' |].
-    + symmetry in Heqval, Heqval2.
-      suff: List.incl u (u ++ [::(i,o)]).
-      * intros Htest.
-        right ; right.
-        exists q, o' ; split ; [auto | split ; [auto | ] ].
-        econstructor.
-        { now apply eval_list_In_is_fun. }
-        right ; left.
-        exists a.
-        revert Heqa.
-        admit.
-      * apply List.incl_appl, List.incl_refl.
-    + left.
-      exists q.
-      split ; [reflexivity | split ; [now auto | ] ].
-      remember (eval_list [::(i,o)] q) as aux ; destruct aux as [o' | ].
-      { cbn in *.
-        destruct (@eqP I q i) as [? | Hnoteq] ; [subst ; assumption | now inversion Heqaux].
-      }
-      symmetry in Heqaux,Heqval,Heqval2 ; apply eval_list_notin in Heqaux.
-      exfalso.
-      eapply (eval_ext_tree_aux_finapp_monotone_ask_fuel 1 Hfun Heqval2) in Heqval.
-      eapply (eval_ext_tree_aux_finapp_monotone_ask_list) in Heqval ; [ | exact Hnodup | | ].
-      * rewrite size_cat Heqval in Heqa ; now inversion Heqa.
-      * now apply List.incl_appl, List.incl_refl.
-      * now apply eval_list_notin_cat.
-  - subst.
-    remember (eval_ext_tree_aux_finapp tau u (size u) nil) as aux.
-    destruct aux as [q' | r].
-    2: econstructor ; [assumption | right ; left ; now exists r ].
-    remember (eval_list u q') as aux2 ; destruct aux2 as [a | ].
-    + econstructor ; [ assumption | ].
-      right ; right ; exists q',a.
-      split ; [now auto | split ; [now auto | ] ].
-      remember (eval_ext_tree_aux_finapp tau (u ++ [:: (q', a)]) (size (u ++ [:: (q', a)])) nil)
-        as aux3.
-      destruct aux3 as [q'' | r].
-      2: econstructor ; [now apply eval_list_In_is_fun | right ; left ; now exists r ].
-      remember (eval_list (u ++ [:: (q', a)]) q'') as aux4 ; destruct aux4 as [a' | ].
-      * suff: q = q''.
-        { intros Heq' ; subst.
-          specialize (IHk i o (u ++ [::(q'', o')])).
-          suff: ext_tree_indbarred
-          
-      
-      unshelve eapply IHk.
-      
-
-      
-    specialize (IHk q o' (u ++ [::(i, o)])).
-*)
-    
-  
-Lemma test (tau : ext_tree) (l : seq (I * O)) (o : O) :
+Lemma indbarred_fun_list_ext_tree_indbarredP_aux
+  (tau : ext_tree) (l : seq (I * O)) (o : O) :
   indbarred_fun_list
     (fun u => exists n a, eval_ext_tree_aux_finapp tau u n nil = output a) l ->
-  ext_tree_indbarredP tau l.
+  ext_tree_indbarredP tau l (size l).
 Proof.
   intros Hyp.
-  assert (aux := indbarred_fun_list_fun_list Hyp) ; revert aux.
+  assert (Hfun := indbarred_fun_list_fun_list Hyp) ; revert Hfun.
   induction Hyp as [u v [n [r Hr]] Hincl Hnodup | q v Hnotin _ IHk].
-  - intros Hfun ; eapply eval_output_indbarredP ; eauto.
-    eapply eval_ext_tree_aux_finapp_monotone_output_list ; now eauto.
+  - intros Hfun ; eapply ext_tree_indbarredP_change_fuel with n ; eauto.
+    eapply eval_output_indbarredP ; eauto.
+    now eapply eval_ext_tree_aux_finapp_monotone_output_list ; eauto.
   - intros Hfun.
-    unshelve eapply super with (v ++ [::(q,o)]) q o.
+    unshelve eapply Add_induction_step with (v ++ [::(q,o)]) q o.
     + rewrite - (cat0s v) ; apply eval_list_notin_cat; auto.
     + rewrite cats1 ; now apply Add_rcons.
-    + apply IHk.
+    + eapply ext_tree_indbarredP_change_fuel.
+      eapply IHk.
       rewrite cats1.
       now apply is_fun_rcons_notin_dom.
     + intros o' w Haddw.
       suff: List.incl (v ++ [:: (q, o')]) w.
       { intros Hincl.
-        eapply ext_tree_indbarredP_monotone ; [ apply IHk | | eassumption].
-        * rewrite cats1.
+        eapply ext_tree_indbarredP_monotone ; [ | | eassumption].
+        * eapply ext_tree_indbarredP_change_fuel, IHk.
+          rewrite cats1.
           now apply is_fun_rcons_notin_dom.
         * apply is_fun_list_incl with (v ++ [::(q, o')]).
           -- rewrite cats1 ; now apply is_fun_rcons_notin_dom.
@@ -1792,68 +1495,26 @@ Proof.
       destruct Hinx ; now left.
 Qed.
 
-Lemma test_noo (tau : ext_tree) (l : seq (I * O)) :
+Lemma indbarred_fun_list_ext_tree_indbarredP (tau : ext_tree) (l : seq (I * O)) :
   indbarred_fun_list
     (fun u => exists n a, eval_ext_tree_aux_finapp tau u n nil = output a) l ->
-  ext_tree_indbarredP tau l.
+  ext_tree_indbarredP tau l (size l).
 Proof.
   destruct l as [ | [i o] l] ; intros Hyp.
-  - econstructor ; [intros i j K H ; inversion H | cbn ].
-    remember (tau nil) as aux ; destruct aux as [q | r] ; [ | right ; left ; now exists r].
-    left ; exists q ; split ; [auto | split ; [auto | ] ].
-    intros o.
-    eapply ext_tree_indbarredP_monotone with nil.
-    + now eapply test.
-    + intros i a a' Hina Hina'.
-      destruct Hina as [H | H] ; inversion H ; subst ; clear H.
-      destruct Hina' as [H | H] ; inversion H ; now subst.
-    + now apply List.incl_nil_l.
-  - eapply test ; eauto.
+  2: now eapply indbarred_fun_list_ext_tree_indbarredP_aux ; eauto.
+  econstructor ; [intros i j K H ; inversion H | cbn ].
+  remember (tau nil) as aux ; destruct aux as [q | r] ; [ | right ; left ; now exists r].
+  left ; exists q ; split ; [auto | split ; [auto | ] ].
+  intros o.
+  eapply ext_tree_indbarredP_monotone with nil.
+  - now eapply indbarred_fun_list_ext_tree_indbarredP_aux.
+  - intros i a a' Hina Hina'.
+    destruct Hina as [H | H] ; inversion H ; subst ; clear H.
+    destruct Hina' as [H | H] ; inversion H ; now subst.
+  - now apply List.incl_nil_l.
 Qed.
   
   
-
-  
-Lemma eval_ext_tree_finapp_trace (tau : ext_tree) f n a l :
-  eval_ext_tree_aux tau f n l = output a ->
-  eval_ext_tree_aux_finapp tau [seq (i, f i) | i <- eval_ext_tree_trace_aux tau f n l]
-    (size (eval_ext_tree_trace_aux tau f n l)) l = output a.
-Proof.
-  assert (aux := @is_fun_map (eval_ext_tree_trace_aux tau f n l) f) ; revert aux.
-  change (eval_ext_tree_trace_aux tau f n l) with (nil ++ (eval_ext_tree_trace_aux tau f n l)) at 1 2.
-  generalize (@nil I) as u ; revert l.
-  induction n as [ | n IHn] ; cbn in * ; intros l u aux Heq.
-  { destruct u ; cbn ; [assumption | now rewrite Heq ]. }
-  remember (tau l) as r ; destruct r ; cbn in *.
-  2:{ destruct u ; cbn ; now rewrite - Heqr. }
-  erewrite <- cat_rcons, <- Heqr ; rewrite - cat_rcons in aux.
-  suff: eval_list [seq (i, f i) | i <- rcons u s ++ eval_ext_tree_trace_aux tau f n (rcons l (f s))] s = Some (f s).
-  { intros Hyp ; rewrite Hyp.
-    specialize (IHn (rcons l (f s)) (rcons u s)) ; erewrite IHn ; [reflexivity | assumption | assumption].
-  }
-Admitted.
-Print deval.
-
-Fixpoint deval_list (d : @dialogue I O A) (l : list (I * O)) : option A :=
-  match d with
-  | eta a => Some a
-  | beta q k => match eval_list l q with
-                | None => None
-                | Some o => deval_list (k o) l
-                end
-  end.
-
-Lemma deval_list_deval d l alpha a:
-  deval_list d [seq (i, alpha i) | i <- l] = Some a ->
-  deval d alpha = a.
-Admitted.
-
-Fixpoint deval_trace (d : @dialogue I O A) f : list (I * O) :=
-  match d with
-  | eta a => nil
-  | beta q k => (q, (f q)) :: (deval_trace (k (f q)) f)
-  end.
-
 
   
 Theorem GBI_GCI F :
@@ -1870,458 +1531,24 @@ Proof.
       eapply eval_ext_tree_output_unique; eauto. 
   }
   unfold GBI in HGBI.
-  pose (T := fun (l : list (I * O)) =>
-               exists d : dialogue,
-                 forall (l' : list (I * O)) (a : A),
-                   List.incl l l' ->
-                    deval_list d l' = Some a <->
-                      eval_ext_tree_aux_finapp tau l' (size l') nil = output a).
+  pose (T:= fun (l : seq (I * O)) =>
+              exists n a, eval_ext_tree_aux_finapp tau l n nil = output a).
   have Help : ABbarred T.
   { intros alpha.
     destruct (HF alpha) as [n Hn].
     exists (eval_ext_tree_trace tau alpha n).
     unfold T.
-    exists (eta (F alpha)).
-    intros l' a Hincl.
-    split ; intros Hyp.
-    + cbn in *.
-      inversion Hyp ; subst ; clear Hyp.
-      admit.
-    + cbn in *.
-      admit.
+    exists n, (F alpha).
+    now eapply eval_ext_tree_finapp_trace.
   }
-  apply HGBI, indbarred_indbarred_NoDup in Help.
-  unfold dialogue_cont.
-  unfold T in * ; clear T.
-  suff: exists d : dialogue, forall (l : list (I * O)) (a : A),
-      List.incl nil l ->
-      deval_list d l = Some a <->
-      eval_ext_tree_aux_finapp tau l (size l) nil = output a.
-
-  { intros [d Hd].
-    exists d ; intros alpha.
-    specialize (HF alpha) as [n Hn].
-    specialize (Hd [seq (i, alpha i) | i <- eval_ext_tree_trace tau alpha n] (F alpha))
-      as [Hd1 Hd2] ; [now apply List.incl_nil_l | ].
-    suff: deval_list d [seq (i, alpha i) | i <- eval_ext_tree_trace tau alpha n] = Some (F alpha).
-    { intros Hyp.
-      symmetry ; eapply deval_list_deval.
-      eassumption.
-    }
-    apply Hd2 ; rewrite size_map.
-    apply eval_ext_tree_finapp_trace ; exact Hn.
-  }
-  revert Help ; clear HF F.
-  generalize (@nil (I * O)).
-  intros l Help.
-  pattern l.
-  induction Help.
-  - destruct H as [d Hd].
-    exists d.
-    intros l' a Hincl.
-    assert (Hincl' := List.incl_tran H0 Hincl).
-    specialize (Hd l' a Hincl') as [Hd1 Hd2] ; split ; intros Hyp.
-    + now apply Hd1.
-    + now apply Hd2.
-  - clear H0.
-    
-    
-    
-    exists d.
-    intros
-  
-  
-  
-  induction Help.
-  
-  
-    
-    2:{ cbn.
-
-  
-  pose (T := fun (l : list (I * O)) =>
-               forall l', List.incl l l' ->
-                          List.NoDup (map fst l') ->
-                          exists a : A,
-                            eval_ext_tree_aux_finapp tau l' (size l') (map snd l) = output a).
-  have Help : ABbarred T.
-  { intros alpha.
-    destruct (HF alpha) as [n Hn].
-    exists (eval_ext_tree_trace tau alpha n).
-    unfold T.
-    intros l' Hincl Hnodup ; exists (F alpha).
-    admit.
-  }
-  apply HGBI, indbarred_indbarred_NoDup in Help.
-  unfold dialogue_cont.
-  
-  induction Help.
-
-  
-  unfold T in * ; clear T.
-  suff: exists d : dialogue, forall alpha : I -> O,
-    exists l : seq (I * O),
-      map alpha (map fst l) = map snd l /\
-        forall l',
-          List.incl l l' ->
-          List.NoDup (map fst l') ->
-          eval_ext_tree_aux_finapp tau l' (size l') (map snd l) = output (deval d alpha).
-  {admit. }
-
-  
-  revert Help HF.
-  unfold eval_ext_tree.
-
-  
-  change (@nil O) with (map snd (@nil (I * O))).
-  generalize (@nil (I * O)) ; intros l Help.
-  pattern l ; induction Help as [u v Hv Hincl Hnodup | ] ; intros HF.
-  - specialize (Hv u Hincl Hnodup) as [a Ha].
-    exists (eta a).
-    intros alpha ; cbn.
-    specialize (HF alpha) as [n Hn].
-    exists v.
-    
-    suff: output (Q := I) (F alpha) = output a by (intros Heq ; inversion Heq).
-    rewrite - Ha ; symmetry.
-    
-
-  
-  suff: exists d : dialogue, forall (alpha : I -> O),
-    exists l, (map alpha (map fst l)) = map snd l /\
-                eval_ext_tree_aux_finapp tau l (size l) nil = output (deval d alpha).
-  { intros [d Hd].
-    exists d.
-    intros alpha.
-    specialize (Hd alpha) as [l [Hl1 Hl2]].
-    admit. }
-  clear HF.
-  have aux: forall alpha, map alpha (map fst (@nil (I * O))) = map snd (@nil (I * O))
-      by reflexivity.
-  revert Help aux.
-  generalize (@nil (I * O)).
-  intros l Help ; pattern l ; induction Help as [u v Hv Hincl Hnodup | ] ; intros aux.
-  - destruct Hv as [a Ha] ; exists (eta a).
-    intros alpha ; cbn ; exists v.
-    split.
-    { admit. }
-    assumption.
-  -
-
-  
-  - revert Hv u Hincl Hnodup.
-    generalize 0 as m.
-    induction v as [ | v x] using last_ind ; intros.
-    { cbn in *.
-      destruct Hv as [a Heqa].
-      exists (eta a) ; intros alpha.
-      exists nil ; cbn.
-      change (map snd u) with (map snd (nil ++ u)) ; rewrite map_cat.
-      now erewrite valid_cat. 
-    }
-    cbn in *.
-(*    remember (tau (map snd u)) as r.
-    destruct r as [ i | ].
-    2:{ exists (eta a) ; intros alpha ; exists 1.
-        cbn ; now rewrite <- Heqr. }
-    cbn in Hv.*)
-    rewrite size_rcons in Hv; cbn in *.
-    remember ( tau [seq i.2 | i <- take m (rcons v x)]) as s.
-    destruct s as [j | a].
-
-    2:{ exfalso.
-        erewrite valid_cat in Heqr.
-        
-    
-
-
-
-
-
-
-
-
-
-
-
-  
-  suff: exists d : dialogue, forall alpha : I -> O,
-      eval_ext_tree_aux_finapp tau (deval_trace d alpha) (size (deval_trace d alpha)) nil =
-        output (deval d alpha).
-  { admit. }
-  clear HF ; unfold T in * ; clear T.
-  revert Help.
-  generalize (@nil (I * O)) ; generalize 0 ; intros n l Help.
-  pattern l.
-  induction Help as [u v [a Ha] Hincl Hnodup | i v Hnotin _ IHk].
-  {
-  2:{
-
-
-    unfold T in *.
-     
-
-  
-  unfold T in * ; clear T.
-  suff: exists d : dialogue, forall (l : list (I * O)) (a : A),
-      deval_list d l = Some a <->
-      eval_ext_tree_aux_finapp tau l (size l) nil = output a.
-
-  { intros [d Hd].
-    exists d ; intros alpha.
-    specialize (HF alpha) as [n Hn].
-    specialize (Hd [seq (i, alpha i) | i <- eval_ext_tree_trace tau alpha n] (F alpha))
-      as [Hd1 Hd2].
-    suff: deval_list d [seq (i, alpha i) | i <- eval_ext_tree_trace tau alpha n] = Some (F alpha).
-    { intros Hyp.
-      symmetry ; eapply deval_list_deval.
-      eassumption.
-    }
-    apply Hd2 ; rewrite size_map.
-    apply eval_ext_tree_finapp_trace ; exact Hn.
-  }
-  clear HF.
-  revert Help.
-  replace (@nil O) with (map snd (take 0 (@nil (I * O)))) by reflexivity.
-  generalize (@nil (I * O)) ; generalize 0 ; intros n l Help.
-  pattern l.
-  induction Help as [u v [a Ha] Hincl Hnodup | i v Hnotin _ IHk].  
-  - admit.
-  - 
-
-    exists (eta a).
-    intros w a'.
-    split ; cbn.
-    { intros Heq ; inversion Heq ; subst.
-      
-    exists (size v) ; cbn.
-    rewrite - Ha.
-
-
-  
-    eapply eval_ext_tree_output_unique ; [eassumption | ].
-    
-    
-      exists n, eval_ext_tree_aux tau alpha n (take 0 nil) = output (deval d alpha).
-  { intros [d Hd].
-    exists d ; intros alpha ; specialize (Hd alpha) as [n Hn] ; [ reflexivity | ].
-    specialize (HF alpha) as [m Hm] ; unfold eval_ext_tree in *.
-    eapply eval_ext_tree_output_unique ; eassumption.
-  }
-  clear HF.
-  revert Help.
-  replace (@nil O) with (map snd (@nil (I * O))) ; change (@nil I) with (map fst (@nil (I * O))).
-  generalize (@nil (I * O)) ; generalize 0 ; intros n l Help.
-  pattern l.
-  induction Help as [u v [a Ha] Hincl Hnodup | i v Hnotin _ IHk].  
-  - exists (eta a).
-    intros alpha Heqalpha.
-    exists (size v) ; cbn.
-    rewrite - Ha.
-    
-
-    revert Hv u Hincl Hnodup.
-    replace (@nil O) with (take 0 (map snd v)) by (now rewrite take0).
-    clear T ; generalize 0 as m.
-    induction v as [ | x] ; intros.
-    { cbn in *.
-      destruct Hv as [a Heqa].
-      exists (eta a) ; intros alpha ; exists 1 ; cbn.
-      unfold valid_ext_tree in Hval.
-      change (map snd u) with (map snd (nil ++ u)) ; rewrite map_cat.
-      now erewrite valid_cat. 
-    }
-    remember (tau (map snd u)) as r.
-    destruct r as [ i | ].
-    2:{ exists (eta a) ; intros alpha ; exists 1.
-        cbn ; now rewrite <- Heqr. }
-    cbn in Hv.
-    remember (tau (take m (x.2 :: [seq i.2 | i <- v]))) as s.
-    destruct s as [j | a].
-    2:{ exfalso.
-        erewrite valid_cat in Heqr.
-        
-
-
-
-
-
-
-
-
-
-
-  
-  
-  pose (T := fun (l : list (I * O)) =>
-               (exists a : A, forall f, map f (map fst l) = map snd l ->
-                                        eval_ext_tree_aux tau f (size l) nil = output a)).
-  have Help : ABbarred T.
-  { intros alpha.
-    destruct (HF alpha) as [n Hn].
-    exists (eval_ext_tree_trace tau alpha n).
-    unfold T.
-    exists (F alpha) ; intros f.
-    erewrite <- (map_comp fst _).
-    erewrite (@eq_map _ _ (fst \o (fun i : I => (i, alpha i))) id) ; [ | now intros k].
-    erewrite map_id, <- (map_comp snd _).
-    erewrite (@eq_map _ _ (snd \o (fun i : I => (i, alpha i))) alpha) ; [ | now intros k].
-    intros Heqf.
-    assert (aux:= eval_ext_tree_trace_size_eval_trace Hn).
-    apply eval_ext_tree_trace_size_eval in Hn ; rewrite <- Hn, size_map ; symmetry.
-    apply eval_ext_tree_continuous.
-    now rewrite - aux.
-  }
-  apply HGBI, indbarred_indbarred_NoDup in Help.
-  unfold dialogue_cont.
-  eapply Delta0_choice in HF as [HF].
-  2:{
-    intros α n. destruct eval_ext_tree eqn:E.
-    - firstorder congruence.
-    - left. destruct (HF α) as [m].
-      f_equal. 
-      eapply eval_ext_tree_output_unique; eauto. 
-  }
-  unfold T in * ; clear T.
-  suff: exists d : dialogue, forall (alpha : I -> O),
-    exists n, eval_ext_tree_aux tau alpha n nil = output (deval d alpha).
-  { intros [d Hd].
-    exists d ; intros alpha ; specialize (Hd alpha) as [n Hn].
-    specialize (HF alpha) as [m Hm] ; unfold eval_ext_tree in *.
-    eapply eval_ext_tree_output_unique ; eassumption.
-  }
-  clear HF.
-  revert Help ; unfold inductively_barred, eval_ext_tree.
-  have aux : forall (f : I -> O), [seq f i | i <- [seq i.1 | i <- (@nil (I * O))]] =
-                                    [seq i.2 | i <- (@nil (I * O))].
-  intros f ; reflexivity.
-  revert aux.
-  generalize (@nil (I * O)) ; intros l Hyp Help ; revert Hyp.
-  pattern l.
-  induction Help as [u v Hv Hincl Hnodup | i v Hnotin _ IHk] ; intros Hyp.
-  
-  - destruct Hv as [a Ha].
-    exists (eta a) ; intros alpha ; exists (size v).
-    cbn.
-    apply Ha.
-    admit.
-  -
-    
-  
-
-
-
-
-  
-  
-  pose (gs := @eval_ext_tree_continuous _ _ _ tau) ; unfold modulus in gs.
-    
-               exists a : A, eval_ext_tree_aux_finapp tau l (size l) nil = output a).
-  have Help : ABbarred T.
-  { intros alpha.
-    destruct (HF alpha) as [n Hn].
-    exists (eval_ext_tree_trace tau alpha n).
-    unfold T.
-    exists (F alpha).
-    rewrite - Hn size_map.
-
-    
-
-  
-    
-    admit.
-  }
-(*    exists (F alpha).
-    rewrite - Hn eval_ext_tree_map.
-    f_equal.
-    erewrite <- map_comp ; apply eq_map.
-    intros i ; reflexivity.
- *)
-  apply HGBI, indbarred_indbarred_NoDup in Help.
-  unfold dialogue_cont.
-  eapply Delta0_choice in HF as [HF].
-  2:{
-    intros α n. destruct eval_ext_tree eqn:E.
-    - firstorder congruence.
-    - left. destruct (HF α) as [m].
-      f_equal. 
-      eapply eval_ext_tree_output_unique; eauto. 
-  }
-  unfold T in * ; clear T.
-  suff: exists d : dialogue, forall (alpha : I -> O),
-    exists l, eval_ext_tree_aux_finapp tau l (size l) nil = output (deval d alpha).
-  { admit. }
-  
-  
-  
-  { intros [b Hb].
-    exists b ; intros alpha; specialize (Hb alpha) as [n Heqn].
-    specialize (HF alpha) as [m Heqm].
-    unfold eval_ext_tree in *.
-    eapply eval_ext_tree_output_unique ; eassumption.
-  }
-  revert Help HF ; unfold inductively_barred, eval_ext_tree.
-  change (@nil O) with (map snd (@nil (I * O))).
-  generalize (@nil (I * O)) ; intros l Help HF.
-
-  clear HF.
-  pattern l.
-  induction Help as [u v Hv Hincl Hnodup | ].
-  - unfold T in Hv.
-    revert Hv u Hincl Hnodup.
-    replace (@nil O) with (take 0 (map snd v)) by (now rewrite take0).
-    clear T ; generalize 0 as m.
-    induction v as [ | x] ; intros.
-    { cbn in *.
-      destruct Hv as [a Heqa].
-      exists (eta a) ; intros alpha ; exists 1 ; cbn.
-      unfold valid_ext_tree in Hval.
-      change (map snd u) with (map snd (nil ++ u)) ; rewrite map_cat.
-      now erewrite valid_cat. 
-    }
-    remember (tau (map snd u)) as r.
-    destruct r as [ i | ].
-    2:{ exists (eta a) ; intros alpha ; exists 1.
-        cbn ; now rewrite <- Heqr. }
-    cbn in Hv.
-    remember (tau (take m (x.2 :: [seq i.2 | i <- v]))) as s.
-    destruct s as [j | a].
-    2:{ exfalso.
-        erewrite valid_cat in Heqr.
-        
-    
-    
-    cbn in *.
-
-      
-
-    unfold T ; intros u ; destruct (tau u) ; [left ; now exists a | right].
-    intros [a Hyp] ; now inversion Hyp.
-  - clear l Help.
-    intros u Hu ; cbn.
-    remember (tau u) as r ; destruct r.
-    + exists (spit a) ; intros alpha ; exists 0 ; now cbn.
-    + exfalso ; destruct Hu as [a Ha] ; rewrite Ha in Heqr.
-      now inversion Heqr.
-  - intros u k IHk ; cbn in *.
-    unshelve eexists.
-    + apply bite ; intros o.
-      exact (proj1_sig (IHk o)).
-    + cbn.
-      intros alpha.
-      destruct (IHk (alpha 0)) as [b IHb].
-      destruct (IHb (alpha \o succn)) as [n Hn] ; cbn in *.
-      exists (S n) ; cbn ; rewrite <- Hn.
-      clear -Hvalid.
-      remember (tau u) as r ; destruct r.
-      * destruct n ; cbn ; [symmetry ; now apply Hvalid |].
-        suff: tau (rcons u (alpha 0)) = Some a by (intros Hyp ; now rewrite Hyp).
-        now apply Hvalid.
-      * generalize 0 ; clear Heqr ; revert alpha u.
-        induction n ; [ reflexivity | cbn ; intros alpha u i].
-        destruct (tau (rcons u (alpha i))) ; [reflexivity |].
-        now eapply IHn.
-Qed.
+  apply HGBI, indbarred_indbarred_fun_list, indbarred_fun_list_ext_tree_indbarredP
+    in Help.
+  eapply ext_tree_indbarred_spec, (ext_tree_indbarred_dialogue Hval) in Help ; auto.
+  destruct Help as [d Hd].
+  exists d ; intros alpha ; specialize (HF alpha) as [n Hn] ; specialize (Hd alpha) as [m Hm].
+  eapply eval_ext_tree_output_unique ; eauto.
+Qed.  
   
   
 End GeneralisedBarInduction.
+.
